Spec. -> Spect.

gathering-nD/RDVinR.v
@@ -111,7 +111,7 @@ Module R := MakeMetricSpace(Rdef).
 Transparent R.origin Rdef.origin R.eq_dec Rdef.eq_dec.
 
 
-(** Small dedicated decision tactic for reals handling 1<>0 and r=r *)
+(** Small dedicated decision tactic for reals handling 1<>0 and and r=r *)
 Ltac Rdec := unfold R.eq_dec, Rdef.eq_dec; repeat
   match goal with
     | |- context[Rdec ?x ?x] =>
@@ -169,7 +169,7 @@ Axiom size_G : nG >= 2.
 Corollary half_size_pos : div2 nG > 0.
 Proof. apply Exp_prop.div2_not_R0. apply size_G. Qed.
 
-
+(** There are nG good robots and no byzantine ones. *)
 Module N : Size with Definition nG := nG with Definition nB := 0.
   Definition nG := nG.
   Definition nB := 0.
@@ -177,13 +177,13 @@ End N.
 
 
 (** The spectrum is a multiset of positions *)
-Module Spec := MultisetSpectrum.Make(R)(N).
+Module Spect := MultisetSpectrum.Make(R)(N).
 
-Notation "s [ pt ]" := (Spec.multiplicity pt s) (at level 5, format "s [ pt ]").
-Notation "!!" := Spec.from_config (at level 1).
-Add Search Blacklist "Spec.M" "Ring".
+Notation "s [ pt ]" := (Spect.multiplicity pt s) (at level 5, format "s [ pt ]").
+Notation "!!" := Spect.from_config (at level 1).
+Add Search Blacklist "Spect.M" "Ring".
 
-Module Export Formalism := Formalism(R)(N)(Spec).
+Module Export Formalism := Formalism(R)(N)(Spect).
 Close Scope R_scope.
 
 (** [gathered_at pos pt] means that in position [pos] all good robots
@@ -204,7 +204,7 @@ Inductive WillGather (pt : R) (e : execution) : Prop :=
     there is no solution to the gathering problem.
     Therefore, we define these positions as [forbidden]. *)
 Definition forbidden (config : Pos.t) :=
-  Nat.Even N.nG /\ let m := Spec.from_config(config) in
+  Nat.Even N.nG /\ let m := Spect.from_config(config) in
   exists pt1 pt2, ~pt1 = pt2 /\ m[pt1] = Nat.div2 N.nG /\ m[pt2] = Nat.div2 N.nG.
 
 (** [solGathering r d] means that any possible (infinite)
@@ -360,12 +360,12 @@ Lemma lift_pos_equiv : forall pos : Pos.t, Pos.eq pos (lift_pos (fun g => pos (G
 Proof. unfold lift_pos. intros pos [g | b]; hnf. reflexivity. now apply Fin.case0. Qed.
 
 (** Spectra can never be empty as the number of robots is non null. *)
-Lemma spec_non_nil : forall conf, ~Spec.eq (!! conf) Spec.empty.
+Lemma spec_non_nil : forall conf, ~Spect.eq (!! conf) Spect.empty.
 Proof.
 intros conf Heq.
-unfold Spec.from_config in Heq.
-rewrite Spec.multiset_empty in Heq.
-assert (Hlgth:= Spec.Pos.list_length conf).
+unfold Spect.from_config in Heq.
+rewrite Spect.multiset_empty in Heq.
+assert (Hlgth:= Spect.Pos.list_length conf).
 rewrite Heq in Hlgth.
 simpl in *.
 unfold N.nG in *.
@@ -373,9 +373,9 @@ assert (hnG:=size_G).
 omega.
 Qed.
 
-Corollary sort_non_nil : forall config, sort (Spec.support (!! config)) <> nil.
+Corollary sort_non_nil : forall config, sort (Spect.support (!! config)) <> nil.
 Proof.
-intros config Habs. apply (spec_non_nil config). rewrite <- Spec.support_nil.
+intros config Habs. apply (spec_non_nil config). rewrite <- Spect.support_nil.
 apply Permutation_nil. setoid_rewrite Permuted_sort at 2. rewrite Habs. reflexivity.
 Qed.
 
@@ -392,40 +392,40 @@ Proof. intros ? ? ? ? ? Hpos. subst. unfold MajTower_at. now setoid_rewrite Hpos
 (** ***  The maximum multiplicity of a multiset  **)
 
 (** [Smax_mult s] returns the maximal multiplicity of configutation [s]. *)
-Definition Smax_mult s := Spec.fold (fun _ => max) s 0%nat.
+Definition Smax_mult s := Spect.fold (fun _ => max) s 0%nat.
 
-Instance Smax_mult_compat : Proper (Spec.eq ==> eq) Smax_mult.
+Instance Smax_mult_compat : Proper (Spect.eq ==> eq) Smax_mult.
 Proof.
-unfold Smax_mult. intros s1 s2 Heq. apply Spec.fold_compat; trivial; refine _.
+unfold Smax_mult. intros s1 s2 Heq. apply Spect.fold_compat; trivial; refine _.
 intros _ _ n m p. do 2 rewrite Nat.max_assoc. now setoid_rewrite Nat.max_comm at 2.
 Qed.
 
 Lemma Smax_mult_map_injective_invariant : forall f, injective eq eq f ->
-  forall s, Smax_mult (Spec.map f s) = Smax_mult s.
+  forall s, Smax_mult (Spect.map f s) = Smax_mult s.
 Proof.
-intros f Hf. apply Spec.ind.
+intros f Hf. apply Spect.ind.
 + intros s1 s2 Hs. now rewrite Hs.
-+ intros s x n Hout Hn Hrec. rewrite Spec.map_add; try now intros ? ? Heq; rewrite Heq.
-  assert (Haux : Spec.elt -> Spec.elt ->
++ intros s x n Hout Hn Hrec. rewrite Spect.map_add; try now intros ? ? Heq; rewrite Heq.
+  assert (Haux : Spect.elt -> Spect.elt ->
             forall n m a : nat, Init.Nat.max m (Init.Nat.max n a) = Init.Nat.max n (Init.Nat.max m a)).
   { intros _ _ n' m' p'. do 2 rewrite Nat.max_assoc. now setoid_rewrite Nat.max_comm at 2. }
-  unfold Smax_mult in *. repeat rewrite Spec.fold_add; trivial; refine _;try now (hnf;auto).
-  - intro Habs. apply Hout. apply Spec.map_In in Habs.
+  unfold Smax_mult in *. repeat rewrite Spect.fold_add; trivial; refine _;try now (hnf;auto).
+  - intro Habs. apply Hout. apply Spect.map_In in Habs.
     * destruct Habs as [y [Heq Hin]].
       apply Hf in Heq; subst; assumption.
     * repeat intro.
       rewrite H0.
       reflexivity.
-+ now rewrite Spec.map_empty.
++ now rewrite Spect.map_empty.
 Qed.
 
-Corollary Smax_mult_similarity_invariant : forall (sim : similarity) s, Smax_mult (Spec.map sim s) = Smax_mult s.
+Corollary Smax_mult_similarity_invariant : forall (sim : similarity) s, Smax_mult (Spect.map sim s) = Smax_mult s.
 Proof. intros. apply Smax_mult_map_injective_invariant. auto. Qed.
 
-Lemma Smax_mult_add : forall s x n, (n > 0)%nat -> ~Spec.In x s ->
-  Smax_mult (Spec.add x n s) = Nat.max n (Smax_mult s).
+Lemma Smax_mult_add : forall s x n, (n > 0)%nat -> ~Spect.In x s ->
+  Smax_mult (Spect.add x n s) = Nat.max n (Smax_mult s).
 Proof.
-intros s x n Hn. unfold Smax_mult. apply Spec.fold_add; trivial.
+intros s x n Hn. unfold Smax_mult. apply Spect.fold_add; trivial.
 - refine _.
 - repeat intro. now subst.
 - repeat intro. do 2 rewrite Nat.max_assoc. now setoid_rewrite Nat.max_comm at 2.
@@ -433,48 +433,48 @@ Qed.
 
 Theorem Smax_mult_spec : forall s x, (s[x] <= Smax_mult s)%nat.
 Proof.
-intro s. pattern s. apply Spec.ind; clear s.
+intro s. pattern s. apply Spect.ind; clear s.
 * intros s1 s2 Hs. now setoid_rewrite Hs.
 * intros m x n Hout Hn Hrec y. rewrite Smax_mult_add; trivial.
-  assert (Hx : m[x] = 0%nat). { rewrite Spec.not_In in Hout. assumption. }
+  assert (Hx : m[x] = 0%nat). { rewrite Spect.not_In in Hout. assumption. }
   destruct (Rdec y x) as [Hxy | Hxy].
-  + subst. rewrite Spec.add_spec, Hx. rewrite Spec.eq_refl_left. apply Max.le_max_l.
-  + rewrite Spec.add_other; auto. transitivity (Smax_mult m).
+  + subst. rewrite Spect.add_spec, Hx. rewrite Spect.eq_refl_left. apply Max.le_max_l.
+  + rewrite Spect.add_other; auto. transitivity (Smax_mult m).
     - apply Hrec.
     - apply Max.le_max_r.
-* intro x. rewrite Spec.empty_spec. omega.
+* intro x. rewrite Spect.empty_spec. omega.
 Qed.
 
-Lemma Smax_mult_0 : forall s, Smax_mult s = 0%nat <-> Spec.eq s Spec.empty.
+Lemma Smax_mult_0 : forall s, Smax_mult s = 0%nat <-> Spect.eq s Spect.empty.
 Proof.
 intro s. split; intro Heq.
-+ destruct (Spec.empty_or_In_dec s) as [? | [x Hin]]; trivial.
++ destruct (Spect.empty_or_In_dec s) as [? | [x Hin]]; trivial.
   elim (lt_irrefl 0). apply lt_le_trans with s[x].
   - exact Hin.
   - rewrite <- Heq. apply Smax_mult_spec.
-+ rewrite Heq. unfold Smax_mult. now rewrite Spec.fold_empty.
++ rewrite Heq. unfold Smax_mult. now rewrite Spect.fold_empty.
 Qed.
 
 (** ***  Elements of a multiset with maximal multiplciity  **)
 
 (** [Smax s] return the configuration [s] where all non maximal positions
     have been removed. *)
-Definition Smax s := Spec.filter (fun _ => beq_nat (Smax_mult s)) s.
+Definition Smax s := Spect.filter (fun _ => beq_nat (Smax_mult s)) s.
 
-Instance Smax_compat : Proper (Spec.eq ==> Spec.eq) Smax.
+Instance Smax_compat : Proper (Spect.eq ==> Spect.eq) Smax.
 Proof.
-intros s1 s2 Heq. unfold Smax. rewrite Heq. apply Spec.filter_extensionality_compat.
+intros s1 s2 Heq. unfold Smax. rewrite Heq. apply Spect.filter_extensionality_compat.
 - repeat intro. now subst.
 - intros _ n. now rewrite Heq.
 Qed.
 
 Lemma Smax_map_injective : forall f, injective eq eq f ->
-  forall s, Spec.eq (Smax (Spec.map f s)) (Spec.map f (Smax s)).
+  forall s, Spect.eq (Smax (Spect.map f s)) (Spect.map f (Smax s)).
 Proof.
-intros f Hf s. unfold Smax. rewrite Spec.map_injective_filter.
-+ apply Spec.map_compat.
+intros f Hf s. unfold Smax. rewrite Spect.map_injective_filter.
++ apply Spect.map_compat.
   - intros ? ? Heq. now rewrite Heq.
-  - apply Spec.filter_extensionality_compat; repeat intro; subst; trivial.
+  - apply Spect.filter_extensionality_compat; repeat intro; subst; trivial.
     now rewrite Smax_mult_map_injective_invariant.
 + repeat intro. now subst.
 + intros ? ? Heq. now rewrite Heq.
@@ -482,86 +482,86 @@ intros f Hf s. unfold Smax. rewrite Spec.map_injective_filter.
 Qed.
 
 Corollary Smax_similarity : forall (sim : similarity),
-  forall s, Spec.eq (Smax (Spec.map sim s)) (Spec.map sim (Smax s)).
+  forall s, Spect.eq (Smax (Spect.map sim s)) (Spect.map sim (Smax s)).
 Proof. intros. apply Smax_map_injective. auto. Qed.
 
 
 Instance eqb_Smax_mult_compat s:
   Proper (R.eq ==> eq ==> eq)
-         (fun _ : Spec.elt => Nat.eqb (Smax_mult s)).
+         (fun _ : Spect.elt => Nat.eqb (Smax_mult s)).
 Proof.
   repeat intro. now subst.
 Qed.
 
 Local Hint Immediate eqb_Smax_mult_compat.
 
-Lemma Smax_subset : forall s, Spec.Subset (Smax s) s.
+Lemma Smax_subset : forall s, Spect.Subset (Smax s) s.
 Proof.
   intros s x.
   unfold Smax.
-  setoid_rewrite Spec.filter_spec.
+  setoid_rewrite Spect.filter_spec.
   2: apply eqb_Smax_mult_compat.
   destruct (Smax_mult s =? s[x]);auto.
   omega.
 Qed.
 
-Theorem Smax_spec1 : forall s x y, Spec.In y (Smax s) -> (s[x] <= (Smax s)[y])%nat.
+Theorem Smax_spec1 : forall s x y, Spect.In y (Smax s) -> (s[x] <= (Smax s)[y])%nat.
 Proof.
 intros s x y Hy. unfold Smax in *.
 (* assert (Hf := eqb_Smax_mult_compat s). *)
-unfold Spec.In in Hy. rewrite Spec.filter_spec in *; auto.
+unfold Spect.In in Hy. rewrite Spect.filter_spec in *; auto.
 destruct (Smax_mult s =? s[y]) eqn:Heq; try omega.
 rewrite Nat.eqb_eq in Heq. rewrite <- Heq. apply Smax_mult_spec.
 Qed.
 
-Theorem Smax_spec_non_nil : forall s x, Spec.In x s -> exists y, Spec.In y (Smax s).
+Theorem Smax_spec_non_nil : forall s x, Spect.In x s -> exists y, Spect.In y (Smax s).
 Proof.
   intro s.
   pattern s.
-  apply Spec.ind.
+  apply Spect.ind.
   - intros m1 m2 Hm1m2. now setoid_rewrite Hm1m2.
   - intros m x n Hxnotinm Hpos HI x' Hx'.
-    destruct (Spec.empty_or_In_dec m).
-    + exists x. unfold Smax. rewrite Spec.filter_In; auto. split.
-      * rewrite Spec.add_In. right. split; reflexivity || omega.
+    destruct (Spect.empty_or_In_dec m).
+    + exists x. unfold Smax. rewrite Spect.filter_In; auto. split.
+      * rewrite Spect.add_In. right. split; reflexivity || omega.
       * rewrite Nat.eqb_eq, Smax_mult_add; trivial.
         rewrite e at 2.
-        rewrite Spec.add_empty, Spec.singleton_spec.
+        rewrite Spect.add_empty, Spect.singleton_spec.
         unfold R.eq_dec,Rdef.eq_dec. Rdec.
         rewrite <- Smax_mult_0 in e. rewrite e.
         apply Max.max_0_r.
     + destruct e as [x'' Hx''].
       specialize (HI x'' Hx'').
       destruct HI as [y Hy]. unfold Smax.
-      setoid_rewrite Spec.filter_In; try now repeat intro; subst.
+      setoid_rewrite Spect.filter_In; try now repeat intro; subst.
       rewrite Smax_mult_add; trivial.
-      unfold Smax in Hy. rewrite Spec.filter_In in Hy; auto.
+      unfold Smax in Hy. rewrite Spect.filter_In in Hy; auto.
       destruct Hy as [Hy Heq]. rewrite Nat.eqb_eq in Heq.
       destruct (le_lt_dec n (m[y])).
       * { exists y. split.
-          - now rewrite Spec.add_In; auto.
-          - rewrite Nat.eqb_eq, Heq, Spec.add_other, Max.max_r; trivial.
+          - now rewrite Spect.add_In; auto.
+          - rewrite Nat.eqb_eq, Heq, Spect.add_other, Max.max_r; trivial.
             intro Habs. apply Hxnotinm. now rewrite <- Habs. }
       * { exists x. split.
-          - rewrite Spec.add_In. right. split; reflexivity || omega.
+          - rewrite Spect.add_In. right. split; reflexivity || omega.
           - rewrite Nat.eqb_eq, Max.max_l; try omega.
-            rewrite Spec.not_In in Hxnotinm. now rewrite Spec.add_same, Hxnotinm. }
-  - intros x H. elim (Spec.In_empty H).
+            rewrite Spect.not_In in Hxnotinm. now rewrite Spect.add_same, Hxnotinm. }
+  - intros x H. elim (Spect.In_empty H).
 Qed.
 
 
-Lemma Smax_empty : forall s, Spec.eq (Smax s) Spec.empty <-> Spec.eq s Spec.empty.
+Lemma Smax_empty : forall s, Spect.eq (Smax s) Spect.empty <-> Spect.eq s Spect.empty.
 Proof.
 intro s. split; intro H.
-- destruct (Spec.empty_or_In_dec s) as [Hs | Hs].
+- destruct (Spect.empty_or_In_dec s) as [Hs | Hs].
   + intro. now rewrite Hs.
   + destruct Hs as [x Hx].
     destruct (Smax_spec_non_nil Hx) as [y Hy].
-    unfold Spec.In in Hy.
-    rewrite H in Hy. rewrite Spec.empty_spec in Hy. omega.
+    unfold Spect.In in Hy.
+    rewrite H in Hy. rewrite Spect.empty_spec in Hy. omega.
 - rewrite H.
   unfold Smax.
-  rewrite Spec.filter_empty.
+  rewrite Spect.filter_empty.
   + reflexivity.
   + intros r1 r2 Hr1r2 x1 x2 hx1x2.
     subst.
@@ -570,59 +570,59 @@ Qed.
 
 Lemma Smax_2_mult : forall s x, (Smax s)[x] = 0 \/ (Smax s)[x] = s[x].
 Proof.
-intros s x. destruct (Spec.empty_or_In_dec s) as [Hs | Hs].
-+ left. rewrite <- Smax_empty in Hs. rewrite (Hs x). apply Spec.empty_spec.
-+ unfold Smax. rewrite Spec.filter_spec.
+intros s x. destruct (Spect.empty_or_In_dec s) as [Hs | Hs].
++ left. rewrite <- Smax_empty in Hs. rewrite (Hs x). apply Spect.empty_spec.
++ unfold Smax. rewrite Spect.filter_spec.
   destruct (Smax_mult s =? s[x]) as [Heq | Heq]; auto.
   repeat intro. now subst.
 Qed.
 (*
-Lemma Smax_val : forall s x, Spec.In x (Smax s) -> s[x] = Smax_mult s.
+Lemma Smax_val : forall s x, Spect.In x (Smax s) -> s[x] = Smax_mult s.
 Proof.
 intros s x Hin.
 Qed.
 *)
-Lemma Smax_In_mult : forall s x, Spec.In x s -> (Spec.In x (Smax s) <-> (Smax s)[x] = s[x]).
-Proof. intros s x Hin. unfold Spec.In in *. destruct (Smax_2_mult s x); omega. Qed.
+Lemma Smax_In_mult : forall s x, Spect.In x s -> (Spect.In x (Smax s) <-> (Smax s)[x] = s[x]).
+Proof. intros s x Hin. unfold Spect.In in *. destruct (Smax_2_mult s x); omega. Qed.
 
-Lemma Smax_spec_mult : forall s x y, Spec.In x (Smax s) -> (Spec.In y (Smax s) <-> (Smax s)[y] = (Smax s)[x]).
+Lemma Smax_spec_mult : forall s x y, Spect.In x (Smax s) -> (Spect.In y (Smax s) <-> (Smax s)[y] = (Smax s)[x]).
 Proof.
 intros s x y Hx. split.
 + intro Hy. destruct (Smax_2_mult s x) as [Hx' | Hx'], (Smax_2_mult s y) as [Hy' | Hy'];
-  (unfold Spec.In in *; omega) || (try congruence); [].
+  (unfold Spect.In in *; omega) || (try congruence); [].
   apply le_antisym.
   - rewrite Hy'. now apply Smax_spec1.
   - rewrite Hx'. now apply Smax_spec1.
-+ intro Heq. unfold Spec.In in *. now rewrite Heq.
++ intro Heq. unfold Spect.In in *. now rewrite Heq.
 Qed.
 
 Theorem Smax_spec2 : forall s x y,
-  Spec.In x (Smax s) -> ~Spec.In y (Smax s) -> (s[y] < s[x])%nat.
+  Spect.In x (Smax s) -> ~Spect.In y (Smax s) -> (s[y] < s[x])%nat.
 Proof.
 intros s x y Hx Hy. apply le_neq_lt.
 + assert (Hx' := Hx). rewrite Smax_In_mult in Hx.
   - rewrite <- Hx. now apply Smax_spec1.
   - now rewrite <- Smax_subset.
-+ intro Habs. apply Hy. unfold Smax. rewrite Spec.filter_In; try now repeat intro; subst. split.
-  - unfold Spec.In in *. rewrite Habs. apply lt_le_trans with (Smax s)[x]; trivial. apply Smax_subset.
-  - rewrite Habs. unfold Smax in Hx. rewrite Spec.filter_In in Hx; try now repeat intro; subst.
++ intro Habs. apply Hy. unfold Smax. rewrite Spect.filter_In; try now repeat intro; subst. split.
+  - unfold Spect.In in *. rewrite Habs. apply lt_le_trans with (Smax s)[x]; trivial. apply Smax_subset.
+  - rewrite Habs. unfold Smax in Hx. rewrite Spect.filter_In in Hx; try now repeat intro; subst.
 Qed.
 
 Close Scope R_scope.
   
-Lemma Smax_max_mult : forall s x, ~Spec.eq s Spec.empty -> Spec.In x (Smax s) <-> s[x] = Smax_mult s.
+Lemma Smax_max_mult : forall s x, ~Spect.eq s Spect.empty -> Spect.In x (Smax s) <-> s[x] = Smax_mult s.
 Proof.
   intros s x hnonempty.
   split.
   - intros H.
-    apply Spec.filter_In in H;auto.
+    apply Spect.filter_In in H;auto.
     destruct H.
     symmetry.
     apply beq_nat_true.
     assumption.
   - intro H.
     unfold Smax.
-    rewrite Spec.filter_In;auto.
+    rewrite Spect.filter_In;auto.
     split.
     + assert (s[x]<>0).
       { intro abs.
@@ -636,29 +636,29 @@ Proof.
       apply beq_nat_refl.
 Qed.
 
-Lemma Smax_max_mult_ex : forall s, ~Spec.eq s Spec.empty -> exists x, Smax_mult s = s[x].
+Lemma Smax_max_mult_ex : forall s, ~Spect.eq s Spect.empty -> exists x, Smax_mult s = s[x].
 Proof.
   intros s.
   pattern s.
-  apply Spec.ind.
+  apply Spect.ind.
   - repeat intro.
     setoid_rewrite H.
     reflexivity.
   - intros m x n H H0 H1 H2.
     clear H2.
-    destruct (Spec.empty_or_In_dec m).
+    destruct (Spect.empty_or_In_dec m).
     exists x.
     rewrite e.
-    rewrite Spec.add_empty.
+    rewrite Spect.add_empty.
     unfold Smax_mult.
-    + rewrite Spec.fold_singleton;auto.
+    + rewrite Spect.fold_singleton;auto.
       * rewrite Max.max_0_r.
         symmetry.
-        apply Spec.singleton_same.
+        apply Spect.singleton_same.
       * repeat intro.
         subst;auto.
-    + assert (~ Spec.eq m Spec.empty).
-      { rewrite Spec.not_empty_In.
+    + assert (~ Spect.eq m Spect.empty).
+      { rewrite Spect.not_empty_In.
         assumption. }
       specialize (H1 H2).
       clear e H2.
@@ -666,17 +666,17 @@ Proof.
       rewrite Smax_mult_add;auto.
       destruct (Max.max_spec n (Smax_mult m)) as [[h_max1 h_max2]|[h_max1 h_max2]].
       * exists max_m.
-        rewrite Spec.add_other.
+        rewrite Spect.add_other.
         -- rewrite <- h_max_m.
            assumption.
         -- intro abs.
            rewrite abs in *.
-           rewrite Spec.not_In in H.
+           rewrite Spect.not_In in H.
            exfalso;omega.
       * exists x.
         rewrite h_max2.
-        rewrite Spec.add_same.
-        rewrite Spec.not_In in H.
+        rewrite Spect.add_same.
+        rewrite Spect.not_In in H.
         omega.
   - intro abs.
     elim abs.
@@ -686,7 +686,7 @@ Qed.
 
 Lemma Smax_spec_max :
   forall s x,
-    ~Spec.eq s Spec.empty ->
+    ~Spect.eq s Spect.empty ->
     (forall y, (s[y] <= s[x])) -> Smax_mult s = s[x].
 Proof.
   intros s x hnonempty h.
@@ -699,14 +699,14 @@ Qed.
 
 
 Corollary Smax_spec1_iff : forall s,
-    ~Spec.eq s Spec.empty ->
+    ~Spect.eq s Spect.empty ->
     forall x,
-      Spec.In x (Smax s) <-> forall y, (s[y] <= s[x]).
+      Spect.In x (Smax s) <-> forall y, (s[y] <= s[x]).
 Proof.
   intros s Hs x.
   assert (h_empty:=Hs).
   rewrite <- Smax_empty in Hs.
-  rewrite Spec.not_empty_In in Hs.
+  rewrite Spect.not_empty_In in Hs.
   destruct Hs as [z Hz].
   split; intro Hx.
   - intro y. assert (Hx' := Hx). rewrite Smax_In_mult in Hx.
@@ -717,29 +717,29 @@ Proof.
 Qed.
 
 
-Lemma support_Smax_non_nil : forall config, Spec.support (Smax (!! config)) <> nil.
-Proof. intros config Habs. rewrite Spec.support_nil, Smax_empty in Habs. apply (spec_non_nil _ Habs). Qed.
+Lemma support_Smax_non_nil : forall config, Spect.support (Smax (!! config)) <> nil.
+Proof. intros config Habs. rewrite Spect.support_nil, Smax_empty in Habs. apply (spec_non_nil _ Habs). Qed.
 
 (** ***  Computational equivalent of having a majority tower  **)
 
 Lemma Majority_MajTower_at : forall config pt,
-  Spec.support (Smax (!! config)) = pt :: nil -> MajTower_at pt config.
+  Spect.support (Smax (!! config)) = pt :: nil -> MajTower_at pt config.
 Proof.
 intros config pt Hmaj x Hx. apply Smax_spec2.
-- rewrite <- Spec.support_In, Hmaj. now left.
-- rewrite <- Spec.support_In, Hmaj. intro Habs. inversion_clear Habs. now auto. inversion H.
+- rewrite <- Spect.support_In, Hmaj. now left.
+- rewrite <- Spect.support_In, Hmaj. intro Habs. inversion_clear Habs. now auto. inversion H.
 Qed.
 
 Theorem MajTower_at_equiv : forall config pt, MajTower_at pt config <->
-  Spec.support (Smax (!! config)) = pt :: nil.
+  Spect.support (Smax (!! config)) = pt :: nil.
 Proof.
 intros config pt. split; intro Hmaj.
 * apply Permutation_length_1_inv. rewrite <- PermutationA_Leibniz.
   apply (NoDupA_equivlistA_PermutationA _).
   + apply NoDupA_singleton.
-  + apply Spec.support_NoDupA.
+  + apply Spect.support_NoDupA.
   + intro y. rewrite InA_singleton.
-    rewrite Spec.support_In, Smax_spec1_iff; try apply spec_non_nil; [].
+    rewrite Spect.support_In, Smax_spec1_iff; try apply spec_non_nil; [].
     split; intro Hpt.
     - subst y. intro x. destruct (Rdec x pt).
       -- subst x. reflexivity.
@@ -749,8 +749,8 @@ intros config pt. split; intro Hmaj.
       eapply le_lt_trans; try eassumption; [].
       apply Hpt.
 * intros x Hx. apply Smax_spec2.
-  - rewrite <- Spec.support_In, Hmaj. now left.
-  - rewrite <- Spec.support_In, Hmaj. intro Habs. inversion_clear Habs. now auto. inversion H.
+  - rewrite <- Spect.support_In, Hmaj. now left.
+  - rewrite <- Spect.support_In, Hmaj. intro Habs. inversion_clear Habs. now auto. inversion H.
 Qed.
 
 (** **  Some properties of [forbidden]  **)
@@ -765,27 +765,27 @@ Lemma forbidden_even : forall pos, forbidden pos -> Nat.Even nG.
 Proof. now intros pos [? _]. Qed.
 
 Lemma forbidden_support_length : forall config, forbidden config ->
-  Spec.size (!! config) = 2.
+  Spect.size (!! config) = 2.
 Proof.
 intros conf [Heven [pt1 [pt2 [Hdiff [Hpt1 Hpt2]]]]].
-rewrite <- (@Spec.cardinal_total_sub_eq (Spec.add pt2 (Nat.div2 N.nG) (Spec.singleton pt1 (Nat.div2 N.nG)))
+rewrite <- (@Spect.cardinal_total_sub_eq (Spect.add pt2 (Nat.div2 N.nG) (Spect.singleton pt1 (Nat.div2 N.nG)))
                                         (!! conf)).
-+ rewrite Spec.size_add; try now apply half_size_pos.
-  destruct (Spec.In_dec pt2 (Spec.singleton pt1 (Nat.div2 N.nG))) as [Hin | Hin].
-  - exfalso. rewrite Spec.In_singleton in Hin.
++ rewrite Spect.size_add; try now apply half_size_pos.
+  destruct (Spect.In_dec pt2 (Spect.singleton pt1 (Nat.div2 N.nG))) as [Hin | Hin].
+  - exfalso. rewrite Spect.In_singleton in Hin.
     destruct Hin. now elim Hdiff.
-  - rewrite Spec.size_singleton; trivial. apply half_size_pos.
+  - rewrite Spect.size_singleton; trivial. apply half_size_pos.
 + intro pt. destruct (Rdec pt pt2), (Rdec pt pt1); subst.
   - now elim Hdiff.
-  - rewrite Spec.add_spec, Spec.singleton_spec.
+  - rewrite Spect.add_spec, Spect.singleton_spec.
     unfold R.eq_dec, Rdef.eq_dec in *. do 2 Rdec_full; contradiction || omega.
-  - rewrite Spec.add_other, Spec.singleton_spec.
+  - rewrite Spect.add_other, Spect.singleton_spec.
       now unfold R.eq_dec, Rdef.eq_dec in *; Rdec_full; contradiction || omega.
       now unfold R.eq, Rdef.eq; auto.
-  - rewrite Spec.add_other, Spec.singleton_spec.
+  - rewrite Spect.add_other, Spect.singleton_spec.
       now unfold R.eq_dec, Rdef.eq_dec in *; Rdec_full; contradiction || omega.
       now unfold R.eq, Rdef.eq; auto.
-+ rewrite Spec.cardinal_add, Spec.cardinal_singleton, Spec.cardinal_from_config.
++ rewrite Spect.cardinal_add, Spect.cardinal_singleton, Spect.cardinal_from_config.
   unfold N.nB.
   replace (Nat.div2 N.nG + Nat.div2 N.nG) with (2 * Nat.div2 N.nG) by lia.
   rewrite <- Nat.double_twice, plus_0_r. symmetry. apply even_double. now rewrite Even.even_equiv.
@@ -799,7 +799,7 @@ intros f Hf pos [HnG [pt1 [pt2 [Hdiff [Hpt1 Hpt2]]]]].
 split;trivial.
 exists (f pt1), (f pt2). split.
 - intro Heq. apply Hdiff. now apply Hf in Heq.
-- split; rewrite <- Spec.from_config_map, Spec.map_injective_spec;
+- split; rewrite <- Spect.from_config_map, Spect.map_injective_spec;
   assumption || (now intros ? ? Heq; rewrite Heq) || apply Hf.
 Qed.
 
@@ -817,26 +817,26 @@ Lemma support_Smax_1_not_forbidden : forall config pt,
   MajTower_at pt config -> ~forbidden config.
 Proof.
 intros config pt Hmaj. rewrite MajTower_at_equiv in Hmaj.
-assert (Hmax : forall x, Spec.In x (Smax (!! config)) <-> x = pt).
-{ intro x. rewrite <- Spec.support_spec, Hmaj. split.
+assert (Hmax : forall x, Spect.In x (Smax (!! config)) <-> x = pt).
+{ intro x. rewrite <- Spect.support_spec, Hmaj. split.
   - intro Hin. inversion_clear Hin. assumption. inversion H.
   - intro. subst x. now left. }
 intro Hforbidden.
 assert (Hsuplen := forbidden_support_length Hforbidden).
 destruct Hforbidden as [Heven [pt1 [pt2 [Hdiff [Hpt1 Hpt2]]]]].
-assert (Hsup : Permutation (Spec.support (!! config)) (pt1 :: pt2 :: nil)).
-{ assert (Hin1 : InA eq pt1 (Spec.support (!! config))).
-  { rewrite Spec.support_spec. unfold Spec.In. rewrite Hpt1. apply half_size_pos. }
-  assert (Hin2 : InA eq pt2 (Spec.support (!! config))).
-  { rewrite Spec.support_spec. unfold Spec.In. rewrite Hpt2. apply half_size_pos. }
+assert (Hsup : Permutation (Spect.support (!! config)) (pt1 :: pt2 :: nil)).
+{ assert (Hin1 : InA eq pt1 (Spect.support (!! config))).
+  { rewrite Spect.support_spec. unfold Spect.In. rewrite Hpt1. apply half_size_pos. }
+  assert (Hin2 : InA eq pt2 (Spect.support (!! config))).
+  { rewrite Spect.support_spec. unfold Spect.In. rewrite Hpt2. apply half_size_pos. }
   apply (PermutationA_split _) in Hin1. destruct Hin1 as [l Hl]. rewrite Hl in Hin2.
   inversion_clear Hin2; try now subst; elim Hdiff.
-  rewrite Spec.size_spec, Hl in Hsuplen. destruct l as [| x [| ? ?]]; simpl in Hsuplen; try omega.
+  rewrite Spect.size_spec, Hl in Hsuplen. destruct l as [| x [| ? ?]]; simpl in Hsuplen; try omega.
   inversion_clear H; (now inversion H0) || subst. now rewrite <- PermutationA_Leibniz. }
 assert (Hpt : pt = pt1 \/ pt = pt2).
 { assert (Hin : In pt (pt1 :: pt2 :: nil)).
-  { rewrite <- Hsup, <- InA_Leibniz, Spec.support_spec,
-            <- (Smax_subset (!! config)), <- Spec.support_spec, Hmaj.
+  { rewrite <- Hsup, <- InA_Leibniz, Spect.support_spec,
+            <- (Smax_subset (!! config)), <- Spect.support_spec, Hmaj.
     now left. }
 inversion_clear Hin; auto. inversion_clear H; auto. inversion H0. }
 apply (lt_irrefl (Nat.div2 N.nG)). destruct Hpt; subst pt.
@@ -845,32 +845,32 @@ apply (lt_irrefl (Nat.div2 N.nG)). destruct Hpt; subst pt.
 - rewrite <- Hpt1 at 1. rewrite <- Hpt2. apply Smax_spec2; now rewrite Hmax.
 Qed.
 
-Definition no_Majority conf := (Spec.size (Smax (!! conf)) > 1)%nat.
+Definition no_Majority conf := (Spect.size (Smax (!! conf)) > 1)%nat.
 
 (* forbidden_support_length already proves the <- direction *)
 Lemma forbidden_equiv : forall conf,
-  forbidden conf <-> no_Majority conf /\ Spec.size (!! conf) = 2%nat.
+  forbidden conf <-> no_Majority conf /\ Spect.size (!! conf) = 2%nat.
 Proof.
   intro conf. unfold no_Majority. split.
   - intro Hforbidden. split.
-    + rewrite Spec.size_spec. destruct (Spec.support (Smax (!! conf))) as [| pt1 [| pt2 l]] eqn:Hmax.
+    + rewrite Spect.size_spec. destruct (Spect.support (Smax (!! conf))) as [| pt1 [| pt2 l]] eqn:Hmax.
       * exfalso. revert Hmax. apply support_Smax_non_nil.
       * exfalso. revert Hmax Hforbidden. rewrite <- MajTower_at_equiv. apply support_Smax_1_not_forbidden.
       * simpl. omega.
     + now apply forbidden_support_length.
-  - intros [Hlen H2]. rewrite Spec.size_spec in *.
-    destruct (Spec.support (!! conf)) as [| pt1 [| pt2 [| ? ?]]] eqn:Hsupp; try (now simpl in H2; omega); [].
+  - intros [Hlen H2]. rewrite Spect.size_spec in *.
+    destruct (Spect.support (!! conf)) as [| pt1 [| pt2 [| ? ?]]] eqn:Hsupp; try (now simpl in H2; omega); [].
     red.
-    assert (Hlen':(Spec.size (Smax (!! conf)) = 2)%nat).
-    { assert (Spec.size (Smax (!! conf)) <= 2)%nat.
+    assert (Hlen':(Spect.size (Smax (!! conf)) = 2)%nat).
+    { assert (Spect.size (Smax (!! conf)) <= 2)%nat.
       { unfold Smax.
-        rewrite <- H2, <- Hsupp, <- Spec.size_spec.
-        apply Spec.size_filter.
+        rewrite <- H2, <- Hsupp, <- Spect.size_spec.
+        apply Spect.size_filter.
         now repeat intro; subst. }
-      rewrite <- Spec.size_spec in Hlen. omega. }
+      rewrite <- Spect.size_spec in Hlen. omega. }
     clear Hlen.
     (* let us reformulate this in a more convenient way *)
-   cut (exists pt0 pt3 : Spec.elt,
+   cut (exists pt0 pt3 : Spect.elt,
       pt0 <> pt3 /\
       (!! conf)[pt0] = Nat.div2 N.nG /\ (!! conf)[pt3] = Nat.div2 N.nG /\ Nat.Even N.nG).
    { intros h.
@@ -880,33 +880,33 @@ Proof.
    split.
     * assert (hnodup:NoDupA R.eq (pt1 :: pt2 :: nil)). {
         rewrite <- Hsupp.
-        apply Spec.support_NoDupA. }
+        apply Spect.support_NoDupA. }
       intro abs.
       subst.
       inversion hnodup;subst.
       elim H1.
       constructor.
       reflexivity.
-    * assert (h:=@Spec.support_filter _ (eqb_Smax_mult_compat (!!conf)) (!! conf)).
-      change (Spec.filter (fun _ : Spec.elt => Nat.eqb (Smax_mult (!! conf))) (!! conf))
+    * assert (h:=@Spect.support_filter _ (eqb_Smax_mult_compat (!!conf)) (!! conf)).
+      change (Spect.filter (fun _ : Spect.elt => Nat.eqb (Smax_mult (!! conf))) (!! conf))
       with (Smax (!!conf)) in h.
-      assert (Hlen'': length (Spec.support (Smax (!! conf))) = length (Spec.support (!! conf))).
-      { rewrite Spec.size_spec in Hlen'. now rewrite Hsupp. }
+      assert (Hlen'': length (Spect.support (Smax (!! conf))) = length (Spect.support (!! conf))).
+      { rewrite Spect.size_spec in Hlen'. now rewrite Hsupp. }
       assert (h2:=@NoDupA_inclA_length_PermutationA
                     _ R.eq _
-                    (Spec.support (Smax (!! conf)))
-                    (Spec.support (!! conf))
-                    (Spec.support_NoDupA _)
-                    (Spec.support_NoDupA _)
+                    (Spect.support (Smax (!! conf)))
+                    (Spect.support (!! conf))
+                    (Spect.support_NoDupA _)
+                    (Spect.support_NoDupA _)
                     h Hlen'').
-      assert (toto:=@Spec.cardinal_from_config conf).
+      assert (toto:=@Spect.cardinal_from_config conf).
       unfold N.nB in toto.
       rewrite <- plus_n_O in toto.
       assert (~ R.eq pt1 pt2). {
         intro abs.
         repeat red in abs.
         rewrite abs in Hsupp.
-        assert (hnodup:=Spec.support_NoDupA (!! conf)).
+        assert (hnodup:=Spect.support_NoDupA (!! conf)).
         rewrite  Hsupp in hnodup.
         inversion hnodup;subst.
         match goal with
@@ -914,28 +914,28 @@ Proof.
         end.
         constructor 1.
         reflexivity. }
-      assert (heq_conf:Spec.eq (!!conf)
-                               (Spec.add pt1 ((!! conf)[pt1])
-                                         (Spec.add pt2 ((!! conf)[pt2]) Spec.empty))).
+      assert (heq_conf:Spect.eq (!!conf)
+                               (Spect.add pt1 ((!! conf)[pt1])
+                                         (Spect.add pt2 ((!! conf)[pt2]) Spect.empty))).
       { red.
         intros x.
         destruct (R.eq_dec x pt1) as [heqxpt1 | hneqxpt1].
         - rewrite heqxpt1.
-          rewrite Spec.add_same.
-          rewrite (Spec.add_other pt2 pt1).
-          + rewrite Spec.empty_spec.
+          rewrite Spect.add_same.
+          rewrite (Spect.add_other pt2 pt1).
+          + rewrite Spect.empty_spec.
             omega.
           + assumption.
-        - rewrite Spec.add_other;auto.
+        - rewrite Spect.add_other;auto.
           destruct (R.eq_dec x pt2) as [heqxpt2 | hneqxpt2].
           + rewrite heqxpt2.
-            rewrite Spec.add_same.
-            rewrite Spec.empty_spec.
+            rewrite Spect.add_same.
+            rewrite Spect.empty_spec.
             omega.
-          + rewrite Spec.add_other;auto.
-            rewrite Spec.empty_spec.
-            rewrite <- Spec.not_In.
-            rewrite <- Spec.support_spec.
+          + rewrite Spect.add_other;auto.
+            rewrite Spect.empty_spec.
+            rewrite <- Spect.not_In.
+            rewrite <- Spect.support_spec.
             rewrite Hsupp.
             intro abs.
             inversion abs;try contradiction;subst.
@@ -943,48 +943,48 @@ Proof.
             rewrite InA_nil in H3.
             assumption. }
       rewrite heq_conf in toto.
-      rewrite Spec.cardinal_fold_elements in toto.
-      assert (fold_left (fun (acc : nat) (xn : Spec.elt * nat) => snd xn + acc)
+      rewrite Spect.cardinal_fold_elements in toto.
+      assert (fold_left (fun (acc : nat) (xn : Spect.elt * nat) => snd xn + acc)
                         ((pt1, (!! conf)[pt1])
                            :: (pt2, (!! conf)[pt2])
                            :: nil) 0
               = N.nG).
       { rewrite <- toto.
-        eapply MMultiset.Preliminary.fold_left_symmetry_PermutationA with (eqA := Spec.eq_pair);auto.
-        - apply Spec.eq_pair_equiv.
+        eapply MMultiset.Preliminary.fold_left_symmetry_PermutationA with (eqA := Spect.eq_pair);auto.
+        - apply Spect.eq_pair_equiv.
         - apply eq_equivalence.
         - repeat intro;subst.
           rewrite H1.
           reflexivity.
         - intros x y z. omega.
         - symmetry.
-          transitivity ((pt1, (!! conf)[pt1]) :: (Spec.elements (Spec.add pt2 (!! conf)[pt2] Spec.empty))).
-          eapply Spec.elements_add_out;auto.
-          + rewrite heq_conf, Spec.add_same. cut ((!! conf)[pt1] > 0). omega.
-            change (Spec.In pt1 (!! conf)). rewrite <- Spec.support_In, Hsupp. now left.
-          + rewrite Spec.add_empty.
-            rewrite Spec.In_singleton.
+          transitivity ((pt1, (!! conf)[pt1]) :: (Spect.elements (Spect.add pt2 (!! conf)[pt2] Spect.empty))).
+          eapply Spect.elements_add_out;auto.
+          + rewrite heq_conf, Spect.add_same. cut ((!! conf)[pt1] > 0). omega.
+            change (Spect.In pt1 (!! conf)). rewrite <- Spect.support_In, Hsupp. now left.
+          + rewrite Spect.add_empty.
+            rewrite Spect.In_singleton.
             intros [abs _].
             contradiction.
           + apply permA_skip.
             * reflexivity.
-            * transitivity ((pt2, (!! conf)[pt2]) :: Spec.elements Spec.empty).
-              eapply Spec.elements_add_out;auto.
-              -- change (Spec.In pt2 (!! conf)). rewrite <- Spec.support_In, Hsupp. now right; left.
-              -- apply Spec.In_empty.
-              -- now rewrite Spec.elements_empty. }
+            * transitivity ((pt2, (!! conf)[pt2]) :: Spect.elements Spect.empty).
+              eapply Spect.elements_add_out;auto.
+              -- change (Spect.In pt2 (!! conf)). rewrite <- Spect.support_In, Hsupp. now right; left.
+              -- apply Spect.In_empty.
+              -- now rewrite Spect.elements_empty. }
       simpl in H0.
       rewrite <- plus_n_O in H0.
 
       assert ((!! conf)[pt2] = (!! conf)[pt1]).
-      { assert (hfilter:= @Spec.filter_In _ (eqb_Smax_mult_compat (!! conf))).
+      { assert (hfilter:= @Spect.filter_In _ (eqb_Smax_mult_compat (!! conf))).
         transitivity (Smax_mult (!! conf)).
         + specialize (hfilter pt2 (!!conf)).
-          replace (Spec.filter (fun _ : Spec.elt => Nat.eqb (Smax_mult (!! conf))) (!!conf))
+          replace (Spect.filter (fun _ : Spect.elt => Nat.eqb (Smax_mult (!! conf))) (!!conf))
           with (Smax (!!conf)) in hfilter.
           * destruct hfilter as [hfilter1 hfilter2].
             destruct hfilter1.
-            -- apply Spec.support_In.
+            -- apply Spect.support_In.
                rewrite h2.
                rewrite Hsupp.
                constructor 2; constructor 1.
@@ -994,11 +994,11 @@ Proof.
                assumption.
           * trivial.
         + specialize (hfilter pt1 (!!conf)).
-          replace (Spec.filter (fun _ : Spec.elt => Nat.eqb (Smax_mult (!! conf))) (!!conf))
+          replace (Spect.filter (fun _ : Spect.elt => Nat.eqb (Smax_mult (!! conf))) (!!conf))
           with (Smax (!!conf)) in hfilter.
           * destruct hfilter as [hfilter1 hfilter2].
             destruct hfilter1.
-            -- apply Spec.support_In.
+            -- apply Spect.support_In.
                rewrite h2.
                rewrite Hsupp.
                constructor 1.
@@ -1035,15 +1035,15 @@ Proof.
 Qed.
 
 Lemma not_forbidden_not_majority_length : forall conf,
-  no_Majority conf -> ~forbidden conf -> (Spec.size (!! conf) >= 3)%nat.
+  no_Majority conf -> ~forbidden conf -> (Spect.size (!! conf) >= 3)%nat.
 Proof.
 intros conf H1 H2.
-assert (Spec.size (!! conf) > 1)%nat.
+assert (Spect.size (!! conf) > 1)%nat.
 { unfold gt. eapply lt_le_trans; try eassumption.
-  do 2 rewrite Spec.size_spec. apply (NoDupA_inclA_length _).
-  - apply Spec.support_NoDupA.
-  - unfold Smax. apply Spec.support_filter. repeat intro. now subst. }
- destruct (Spec.size (!! conf)) as [| [| [| ?]]] eqn:Hlen; try omega.
+  do 2 rewrite Spect.size_spec. apply (NoDupA_inclA_length _).
+  - apply Spect.support_NoDupA.
+  - unfold Smax. apply Spect.support_filter. repeat intro. now subst. }
+ destruct (Spect.size (!! conf)) as [| [| [| ?]]] eqn:Hlen; try omega.
 exfalso. apply H2. now rewrite forbidden_equiv.
 Qed.
 
@@ -1051,39 +1051,39 @@ Qed.
 
 Open Scope R_scope.
 
-Definition mini s := List.hd 0 (sort (Spec.support s)).
-Definition maxi s := List.last (sort (Spec.support s)) 0.
-Definition middle s := nth 1 (sort (Spec.support s)) 0.
+Definition mini s := List.hd 0 (sort (Spect.support s)).
+Definition maxi s := List.last (sort (Spect.support s)) 0.
+Definition middle s := nth 1 (sort (Spect.support s)) 0.
 
-Instance mini_compat : Proper (Spec.eq ==> eq) mini.
+Instance mini_compat : Proper (Spect.eq ==> eq) mini.
 Proof. intros s1 s2 Hs. unfold mini. now rewrite Hs. Qed.
 
-Instance maxi_compat : Proper (Spec.eq ==> eq) maxi.
+Instance maxi_compat : Proper (Spect.eq ==> eq) maxi.
 Proof. intros s1 s2 Hs. unfold maxi. now rewrite Hs. Qed.
 
-Instance middle_compat : Proper (Spec.eq ==> eq) middle.
+Instance middle_compat : Proper (Spect.eq ==> eq) middle.
 Proof. intros s1 s2 Hs. unfold middle. now rewrite Hs. Qed.
 
-Definition is_extremal r (s : Spec.t) :=
+Definition is_extremal r (s : Spect.t) :=
   if Rdec r (mini s) then true else
   if Rdec r (maxi s) then true else false.
 
-Instance is_extremal_compat : Proper (eq ==> Spec.eq ==> eq) is_extremal.
+Instance is_extremal_compat : Proper (eq ==> Spect.eq ==> eq) is_extremal.
 Proof.
 intros x y ? s s' Hs. subst y. unfold is_extremal, mini, maxi.
-destruct (Rdec x (hd 0 (sort (Spec.support s)))), (Rdec x (hd 0 (sort (Spec.support s'))));
+destruct (Rdec x (hd 0 (sort (Spect.support s)))), (Rdec x (hd 0 (sort (Spect.support s'))));
 try rewrite Hs in *; contradiction || trivial.
-destruct (Rdec x (last (sort (Spec.support s)) 0)), (Rdec x (last (sort (Spec.support s')) 0));
+destruct (Rdec x (last (sort (Spect.support s)) 0)), (Rdec x (last (sort (Spect.support s')) 0));
 try rewrite Hs in *; contradiction || reflexivity.
 Qed.
 
 Lemma is_extremal_map_monotonic_invariant : forall f, monotonic Rleb Rleb f -> injective eq eq f ->
-  forall x config, is_extremal (f x) (Spec.map f (!! config)) = is_extremal x (!! config).
+  forall x config, is_extremal (f x) (Spect.map f (!! config)) = is_extremal x (!! config).
 Proof.
 intros f Hfmon Hfinj x config. unfold is_extremal, mini, maxi.
 assert (Hf : Proper (R.eq ==> R.eq) f). { unfold R.eq, Rdef.eq. repeat intro. now subst. }
 destruct Hfmon as [Hfinc | Hfdec].
-* repeat Rdec_full; trivial; rewrite Spec.map_injective_support, (sort_map_increasing Hfinc) in *; trivial.
+* repeat Rdec_full; trivial; rewrite Spect.map_injective_support, (sort_map_increasing Hfinc) in *; trivial.
   + rewrite (hd_indep _ (f 0)) in Heq.
     - rewrite map_hd in Heq. apply Hfinj in Heq. contradiction.
     - intro Habs. apply map_eq_nil in Habs. now apply (sort_non_nil config).
@@ -1096,7 +1096,7 @@ destruct Hfmon as [Hfinc | Hfdec].
   + rewrite (last_indep _ (f 0)) in Hneq0.
     - elim Hneq0. rewrite map_last. now f_equal.
     - intro Habs. apply map_eq_nil in Habs. now apply (sort_non_nil config).
-* repeat Rdec_full; trivial;rewrite Spec.map_injective_support, (sort_map_decreasing Hfdec) in *; trivial.
+* repeat Rdec_full; trivial;rewrite Spect.map_injective_support, (sort_map_decreasing Hfdec) in *; trivial.
   + rewrite (hd_indep _ (f 0)) in Heq.
     - rewrite hd_rev_last, map_last in Heq. apply Hfinj in Heq. contradiction.
     - intro Habs. rewrite rev_nil in Habs. apply map_eq_nil in Habs. now apply (sort_non_nil config).
@@ -1112,7 +1112,7 @@ destruct Hfmon as [Hfinc | Hfdec].
 Qed.
 
 Corollary is_extremal_similarity_invariant : forall (sim : similarity) config r,
-  is_extremal (sim r) (Spec.map sim (!! config)) = is_extremal r (!! config).
+  is_extremal (sim r) (Spect.map sim (!! config)) = is_extremal r (!! config).
 Proof.
 intros sim pos r. apply is_extremal_map_monotonic_invariant.
 - apply similarity_monotonic.
@@ -1120,22 +1120,22 @@ intros sim pos r. apply is_extremal_map_monotonic_invariant.
 Qed.
 
 (* When there is no robot (s is empty), the center is 0. *)
-Definition extreme_center (s : Spec.t) := (mini s + maxi s) / 2.
+Definition extreme_center (s : Spect.t) := (mini s + maxi s) / 2.
 
-Instance extreme_center_compat : Proper (Spec.eq ==> eq) extreme_center.
+Instance extreme_center_compat : Proper (Spect.eq ==> eq) extreme_center.
 Proof. intros s s' Hs. unfold extreme_center, mini, maxi. now rewrite Hs. Qed.
 
-Lemma extreme_center_similarity : forall (sim : similarity) s, ~Spec.eq s Spec.empty ->
-  extreme_center (Spec.map sim s) = sim (extreme_center s).
+Lemma extreme_center_similarity : forall (sim : similarity) s, ~Spect.eq s Spect.empty ->
+  extreme_center (Spect.map sim s) = sim (extreme_center s).
 Proof.
 intros sim s Hs.
 assert (Hsim1 : Proper (R.eq ==> R.eq) sim). { intros x y Hxy. now rewrite Hxy. }
 assert (Hsim2 := similarity_injective sim).
 unfold extreme_center, mini, maxi.
 destruct (similarity_monotonic sim) as [Hinc | Hdec].
-* rewrite Spec.map_injective_support, (sort_map_increasing Hinc); trivial.
-  assert (Hperm := Permuted_sort (Spec.support s)). destruct (sort (Spec.support s)) as [| x l'].
-  + symmetry in Hperm. apply Permutation_nil in Hperm. elim Hs. now rewrite <- Spec.support_nil.
+* rewrite Spect.map_injective_support, (sort_map_increasing Hinc); trivial.
+  assert (Hperm := Permuted_sort (Spect.support s)). destruct (sort (Spect.support s)) as [| x l'].
+  + symmetry in Hperm. apply Permutation_nil in Hperm. elim Hs. now rewrite <- Spect.support_nil.
   + clear s Hs Hperm. simpl hd. cut (x :: l' <> nil). generalize (x :: l'). intro l.
     generalize 0. induction l; intros r Hl.
     - now elim Hl.
@@ -1143,10 +1143,10 @@ destruct (similarity_monotonic sim) as [Hinc | Hdec].
         simpl. symmetry. now apply similarity_middle.
         rewrite <- IHl. reflexivity. discriminate.
     - discriminate.
-* rewrite Spec.map_injective_support, (sort_map_decreasing Hdec); trivial.
+* rewrite Spect.map_injective_support, (sort_map_decreasing Hdec); trivial.
   rewrite last_rev_hd, hd_rev_last.
-  assert (Hperm := Permuted_sort (Spec.support s)). destruct (sort (Spec.support s)) as [| x l'].
-  + symmetry in Hperm. apply Permutation_nil in Hperm. elim Hs. now rewrite <- Spec.support_nil.
+  assert (Hperm := Permuted_sort (Spect.support s)). destruct (sort (Spect.support s)) as [| x l'].
+  + symmetry in Hperm. apply Permutation_nil in Hperm. elim Hs. now rewrite <- Spect.support_nil.
   + clear s Hs Hperm. simpl hd. cut (x :: l' <> nil). generalize (x :: l'). intro l.
     generalize 0. induction l; intros r Hl.
     - now elim Hl.
@@ -1158,7 +1158,7 @@ destruct (similarity_monotonic sim) as [Hinc | Hdec].
 Qed.
 
 Lemma extreme_center_similarity_invariant : forall (sim : similarity) config,
-  extreme_center (Spec.map sim (!! config)) = sim (extreme_center (!! config)).
+  extreme_center (Spect.map sim (!! config)) = sim (extreme_center (!! config)).
 Proof. intros. apply extreme_center_similarity. apply spec_non_nil. Qed.
 
 
@@ -1172,26 +1172,26 @@ Proof. intros. apply extreme_center_similarity. apply spec_non_nil. Qed.
 **)
 
 
-Definition robogram_pgm (s : Spec.t) : R.t :=
-  match Spec.support (Smax s) with
+Definition robogram_pgm (s : Spect.t) : R.t :=
+  match Spect.support (Smax s) with
     | nil => 0 (* only happen with no robots *)
     | pt :: nil => pt (* case 1: one majority stack *)
     | _ => (* several majority stacks *)
-           if beq_nat (Spec.size s) 3
+           if beq_nat (Spect.size s) 3
            then middle s else
            if is_extremal 0 s then 0 else extreme_center s
   end.
 
 (** The robogram is invariant by permutation of spectra. *)
-Instance robogram_pgm_compat : Proper (Spec.eq ==> eq) robogram_pgm.
+Instance robogram_pgm_compat : Proper (Spect.eq ==> eq) robogram_pgm.
 Proof.
-unfold robogram_pgm. intros s s' Hs. assert (Hperm := Spec.support_compat (Smax_compat Hs)).
-destruct (Spec.support (Smax s)) as [| pt [| pt2 l]].
+unfold robogram_pgm. intros s s' Hs. assert (Hperm := Spect.support_compat (Smax_compat Hs)).
+destruct (Spect.support (Smax s)) as [| pt [| pt2 l]].
 + now rewrite (PermutationA_nil _ Hperm).
 + symmetry in Hperm. destruct (PermutationA_length1 _ Hperm) as [pt' [Heq Hin]]. now rewrite Hin.
 + assert (Hlength := PermutationA_length _ Hperm).
-  destruct (Spec.support (Smax s')) as [| pt' [| pt2' l']]; try discriminate. rewrite Hs.
-  destruct (Spec.size s' =? 3); rewrite Hs; trivial.
+  destruct (Spect.support (Smax s')) as [| pt' [| pt2' l']]; try discriminate. rewrite Hs.
+  destruct (Spect.size s' =? 3); rewrite Hs; trivial.
   destruct (is_extremal 0 s'); try rewrite Hs; reflexivity.
 Qed.
 
@@ -1206,12 +1206,12 @@ Lemma round_simplify : forall da pos,
                       | None => pos id
                       | Some f =>
                           let s := !! pos in
-                          match Spec.support (Smax s) with
+                          match Spect.support (Smax s) with
                             | nil => pos id (* only happen with no robots *)
                             | pt :: nil => pt (* case 1: one majority stack *)
                             | _ => (* several majority stacks *)
-                                   if beq_nat (Spec.size s) 3
-                                   then List.nth 1 (sort (Spec.support s)) 0 else
+                                   if beq_nat (Spect.size s) 3
+                                   then List.nth 1 (sort (Spect.support s)) 0 else
                                    if is_extremal (pos id) s then (pos id) else extreme_center s
                           end
                     end).
@@ -1229,11 +1229,11 @@ assert(Hsimccompat : Proper (R.eq ==> R.eq) (simc pt)). { intros ? ? Heq. now re
 assert (Hsim_inj : injective R.eq R.eq (simc pt)) by now apply similarity_injective.
 (* Unfold the robogram *)
 unfold robogram, robogram_pgm. simpl.
-assert (Hperm : PermutationA R.eq (Spec.support (Smax (!! (Pos.map (simc pt) pos))))
-                                  (List.map (simc pt) (Spec.support (Smax (!! pos))))).
-{ rewrite <- Spec.map_injective_support; trivial. f_equiv.
-  rewrite <- Smax_similarity, Spec.from_config_map; auto. reflexivity. }
-destruct (Spec.support (Smax (!! pos))) as [| pt' [| pt2' l']].
+assert (Hperm : PermutationA R.eq (Spect.support (Smax (!! (Pos.map (simc pt) pos))))
+                                  (List.map (simc pt) (Spect.support (Smax (!! pos))))).
+{ rewrite <- Spect.map_injective_support; trivial. f_equiv.
+  rewrite <- Smax_similarity, Spect.from_config_map; auto. reflexivity. }
+destruct (Spect.support (Smax (!! pos))) as [| pt' [| pt2' l']].
 * (* Empty support *)
   simpl in Hperm. symmetry in Hperm. apply (PermutationA_nil _) in Hperm. rewrite Hperm.
   rewrite da.(step_center); try eassumption. hnf. field. lra.
@@ -1242,15 +1242,15 @@ destruct (Spec.support (Smax (!! pos))) as [| pt' [| pt2' l']].
   hnf in Hy |- *. subst y. rewrite Hsim. field. lra.
 * (* No majority stack *)
   apply (PermutationA_length _) in Hperm.
-  destruct (Spec.support (Smax (!! (Pos.map (simc pt) pos)))) as [| pt'' [| pt2'' l'']];
+  destruct (Spect.support (Smax (!! (Pos.map (simc pt) pos)))) as [| pt'' [| pt2'' l'']];
   try discriminate Hperm. clear Hperm pt' pt2' l' pt'' pt2'' l''.
-  assert (Hlength : Spec.size (!! (Pos.map (simc pt) pos)) = Spec.size (!! pos)).
-  { rewrite <- Spec.from_config_map; trivial. now apply Spec.map_injective_size. }
-  rewrite Hlength. destruct (Spec.size (!! pos) =? 3) eqn:Hlen.
+  assert (Hlength : Spect.size (!! (Pos.map (simc pt) pos)) = Spect.size (!! pos)).
+  { rewrite <- Spect.from_config_map; trivial. now apply Spect.map_injective_size. }
+  rewrite Hlength. destruct (Spect.size (!! pos) =? 3) eqn:Hlen.
   + (* There are three towers *)
-    unfold middle. rewrite <- Spec.from_config_map, Spec.map_injective_support; trivial.
-    rewrite Spec.size_spec in Hlen.
-    destruct (Spec.support (!! pos)) as [| pt1 [| pt2 [| pt3 [| ? ?]]]]; try discriminate Hlen.
+    unfold middle. rewrite <- Spect.from_config_map, Spect.map_injective_support; trivial.
+    rewrite Spect.size_spec in Hlen.
+    destruct (Spect.support (!! pos)) as [| pt1 [| pt2 [| pt3 [| ? ?]]]]; try discriminate Hlen.
     destruct (similarity_monotonic (simc pt)) as [Hinc | Hdec].
     - rewrite (sort_map_increasing Hinc), (nth_indep _ 0 (simc pt 0)),
               map_nth, <- Hinvsim, <- (simc pt).(Inversion); try reflexivity.
@@ -1264,12 +1264,12 @@ destruct (Spec.support (Smax (!! pos))) as [| pt' [| pt2' l']].
         + rewrite map_length, <- Permuted_sort. simpl. exists 1%nat. omega. }
   + (* Generic case *)
     change 0 with R.origin. rewrite <- (simc pt).(center_prop) at 1.
-    rewrite <- Spec.from_config_map, is_extremal_similarity_invariant, da.(step_center); try eassumption.
+    rewrite <- Spect.from_config_map, is_extremal_similarity_invariant, da.(step_center); try eassumption.
     destruct (is_extremal pt (!! pos)).
     - (* The current robot is exremal *)
       hnf. unfold R.origin, Rdef.origin. field. lra.
     - (* The current robot is not exremal *)
-      rewrite <- Spec.from_config_map, extreme_center_similarity; apply spec_non_nil || trivial.
+      rewrite <- Spect.from_config_map, extreme_center_similarity; apply spec_non_nil || trivial.
       hnf. rewrite <- (da.(step_center) _ _ pt Hstep) at 2. now rewrite <- Hinvsim, <- (simc pt).(Inversion).
 Qed.
 
@@ -1287,31 +1287,31 @@ Proof.
 intros da conf pt Hmaj id. rewrite round_simplify.
 rewrite MajTower_at_equiv in Hmaj.
 destruct (step da id); try reflexivity. cbv zeta.
-destruct (Spec.support (Smax (!! conf))) as [| ? [| ? ?]]; try discriminate Hmaj.
+destruct (Spect.support (Smax (!! conf))) as [| ? [| ? ?]]; try discriminate Hmaj.
 inversion Hmaj. reflexivity.
 Qed.
 
 (** If we have three towers, everyone goes to the middle one. **)
 Lemma round_simplify_Three : forall da conf,
   no_Majority conf ->
-  (Spec.size (!! conf) = 3)%nat ->
+  (Spect.size (!! conf) = 3)%nat ->
   Pos.eq (round robogram da conf)
          (fun id => match step da id with
                       | None => conf id
-                      | Some _ => nth 1 (sort (Spec.support (!!  conf))) 0
+                      | Some _ => nth 1 (sort (Spect.support (!!  conf))) 0
                     end).
 Proof.
 intros da pos Hmaj H3 id. rewrite round_simplify.
 destruct (step da id); try reflexivity. cbv zeta.
-unfold no_Majority in Hmaj. rewrite Spec.size_spec in Hmaj.
-destruct (Spec.support (Smax (!! pos))) as [| ? [| ? ?]]; simpl in Hmaj; try omega.
+unfold no_Majority in Hmaj. rewrite Spect.size_spec in Hmaj.
+destruct (Spect.support (Smax (!! pos))) as [| ? [| ? ?]]; simpl in Hmaj; try omega.
 rewrite <- Nat.eqb_eq in H3. rewrite H3. reflexivity.
 Qed.
 
 (** In the general case, all non extremal robots go to the middle of the extreme. *)
 Lemma round_simplify_Generic : forall da conf,
   no_Majority conf ->
-  (Spec.size (!! conf) <> 3)%nat ->
+  (Spect.size (!! conf) <> 3)%nat ->
   Pos.eq (round robogram da conf)
          (fun id => match step da id with
                       | None => conf id
@@ -1321,8 +1321,8 @@ Lemma round_simplify_Generic : forall da conf,
 Proof.
 intros da pos Hmaj H3 id. rewrite round_simplify.
 destruct (step da id); try reflexivity. cbv zeta.
-unfold no_Majority in Hmaj. rewrite Spec.size_spec in Hmaj.
-destruct (Spec.support (Smax (!! pos))) as [| ? [| ? ?]]; simpl in Hmaj; try omega.
+unfold no_Majority in Hmaj. rewrite Spect.size_spec in Hmaj.
+destruct (Spect.support (Smax (!! pos))) as [| ? [| ? ?]]; simpl in Hmaj; try omega.
 rewrite <- Nat.eqb_neq in H3. rewrite H3. reflexivity.
 Qed.
 
@@ -1337,8 +1337,8 @@ Theorem Majority_grow :  forall pt config da, MajTower_at pt config ->
 Proof.
 intros pt pos da Hmaj.
 rewrite (round_simplify_Majority _ Hmaj).
-do 2 rewrite Spec.from_config_spec, Spec.Pos.list_spec.
-induction Spec.Names.names as [| id l]; simpl.
+do 2 rewrite Spect.from_config_spec, Spect.Pos.list_spec.
+induction Spect.Names.names as [| id l]; simpl.
 + reflexivity.
 + destruct (step da id).
   - Rdec. Rdec_full; apply le_n_S + apply le_S; apply IHl.
@@ -1351,8 +1351,8 @@ Theorem Majority_wither : forall pt pt' pos da, pt <> pt' ->
 Proof.
 intros pt pt' pos da Hdiff Hmaj.
 rewrite (round_simplify_Majority _ Hmaj).
-do 2 rewrite Spec.from_config_spec, Spec.Pos.list_spec.
-induction Spec.Names.names as [| id l]; simpl.
+do 2 rewrite Spect.from_config_spec, Spect.Pos.list_spec.
+induction Spect.Names.names as [| id l]; simpl.
 + reflexivity.
 + destruct (step da id).
   - Rdec_full; try contradiction. Rdec_full; try apply le_S; apply IHl.
@@ -1371,7 +1371,7 @@ Qed.
 Theorem Majority_not_forbidden : forall pt config, MajTower_at pt config -> ~forbidden config.
 Proof.
 intros pt config Hmaj. rewrite forbidden_equiv. unfold no_Majority. intros [Hmaj' _].
-rewrite MajTower_at_equiv in Hmaj. rewrite Spec.size_spec, Hmaj in Hmaj'. simpl in *. omega.
+rewrite MajTower_at_equiv in Hmaj. rewrite Spect.size_spec, Hmaj in Hmaj'. simpl in *. omega.
 Qed.
 
 (** **  Properties in the generic case  **)
@@ -1394,11 +1394,11 @@ Lemma Generic_min_max_lt : forall config,
   no_Majority config -> mini (!! config) < maxi (!! config).
 Proof.
 intros config Hmaj. apply Generic_min_max_lt_aux.
-+ apply lt_le_trans with (Spec.size (Smax (!! config))); trivial.
-  rewrite Spec.size_spec. apply (NoDupA_inclA_length _).
-  - apply Spec.support_NoDupA.
-  - apply Spec.support_filter. repeat intro. now subst.
-+ apply Spec.support_NoDupA.
++ apply lt_le_trans with (Spect.size (Smax (!! config))); trivial.
+  rewrite Spect.size_spec. apply (NoDupA_inclA_length _).
+  - apply Spect.support_NoDupA.
+  - apply Spect.support_filter. repeat intro. now subst.
++ apply Spect.support_NoDupA.
 Qed.
 
 Corollary Generic_min_mid_lt : forall config,
@@ -1410,14 +1410,14 @@ Corollary Generic_mid_max_lt : forall config,
 Proof. intros ? H. unfold extreme_center. apply Generic_min_max_lt in H. lra. Qed.
 
 Theorem Generic_min_same : forall da conf,
-  no_Majority conf -> (Spec.size (!! conf) <> 3)%nat ->
+  no_Majority conf -> (Spect.size (!! conf) <> 3)%nat ->
   mini (!! (round robogram da conf)) = mini (!! conf).
 Proof.
 intros da config Hmaj Hlen.
 (* We have a robot [id] at the minimal position in the original config. *)
 assert (Hhdin := sort_non_nil config). apply (hd_In 0%R) in Hhdin.
 rewrite <- Permuted_sort in Hhdin at 2.
-rewrite <- InA_Leibniz, Spec.support_In, Spec.from_config_In in Hhdin.
+rewrite <- InA_Leibniz, Spect.support_In, Spect.from_config_In in Hhdin.
 destruct Hhdin as [id Hid].
 (* Its position before and after are the same *)
 assert (config id = round robogram da config id).
@@ -1428,31 +1428,31 @@ assert (config id = round robogram da config id).
 (** Main proof *)
 apply Rle_antisym.
 * apply sort_min.
-  rewrite <- Hid, <- InA_Leibniz, Spec.support_In, H. apply Spec.pos_in_config.
+  rewrite <- Hid, <- InA_Leibniz, Spect.support_In, H. apply Spect.pos_in_config.
 * apply sort_min.
-  rewrite <- InA_Leibniz, Spec.support_In. apply Spec.from_config_In.
+  rewrite <- InA_Leibniz, Spect.support_In. apply Spect.from_config_In.
   exists id. apply min_sort.
-  + rewrite H, <- InA_Leibniz, Spec.support_In. apply Spec.pos_in_config.
-  + intros y Hy. rewrite <- InA_Leibniz, Spec.support_In, Spec.from_config_In in Hy.
+  + rewrite H, <- InA_Leibniz, Spect.support_In. apply Spect.pos_in_config.
+  + intros y Hy. rewrite <- InA_Leibniz, Spect.support_In, Spect.from_config_In in Hy.
     destruct Hy as [id' Hid']. rewrite <- Hid', Hid.
     rewrite round_simplify_Generic; trivial; [].
     destruct (step da id').
     - unfold is_extremal. repeat Rdec_full.
-      -- apply sort_min. rewrite <- InA_Leibniz, Spec.support_In. apply Spec.pos_in_config.
-      -- apply sort_min. rewrite <- InA_Leibniz, Spec.support_In. apply Spec.pos_in_config.
+      -- apply sort_min. rewrite <- InA_Leibniz, Spect.support_In. apply Spect.pos_in_config.
+      -- apply sort_min. rewrite <- InA_Leibniz, Spect.support_In. apply Spect.pos_in_config.
       -- apply Rlt_le. change (mini (!! config) < extreme_center (!! config)). now apply Generic_min_mid_lt.
-    - apply sort_min. rewrite <- InA_Leibniz, Spec.support_In. apply Spec.pos_in_config.
+    - apply sort_min. rewrite <- InA_Leibniz, Spect.support_In. apply Spect.pos_in_config.
 Qed.
 
 Theorem Generic_max_same : forall da conf,
-  no_Majority conf -> (Spec.size (!! conf) <> 3)%nat ->
+  no_Majority conf -> (Spect.size (!! conf) <> 3)%nat ->
   maxi (!! (round robogram da conf)) = maxi (!! conf).
 Proof.
 intros da config Hmaj Hlen.
 (* We have a robot [id] at the minimal position in the original config. *)
 assert (Hlastin := sort_non_nil config). apply (last_In 0%R) in Hlastin.
 rewrite <- Permuted_sort in Hlastin at 2.
-rewrite <- InA_Leibniz, Spec.support_In, Spec.from_config_In in Hlastin.
+rewrite <- InA_Leibniz, Spect.support_In, Spect.from_config_In in Hlastin.
 destruct Hlastin as [id Hid].
 (* Its position before and after are the same *)
 assert (config id = round robogram da config id).
@@ -1463,25 +1463,25 @@ assert (config id = round robogram da config id).
 (** Main proof *)
 apply Rle_antisym.
 * apply sort_max.
-  rewrite <- InA_Leibniz, Spec.support_In. apply Spec.from_config_In.
+  rewrite <- InA_Leibniz, Spect.support_In. apply Spect.from_config_In.
   exists id. apply max_sort.
-  + rewrite H, <- InA_Leibniz, Spec.support_In. apply Spec.pos_in_config.
-  + intros y Hy. rewrite <- InA_Leibniz, Spec.support_In, Spec.from_config_In in Hy.
+  + rewrite H, <- InA_Leibniz, Spect.support_In. apply Spect.pos_in_config.
+  + intros y Hy. rewrite <- InA_Leibniz, Spect.support_In, Spect.from_config_In in Hy.
     destruct Hy as [id' Hid']. rewrite <- Hid', Hid.
     rewrite round_simplify_Generic; trivial; [].
     destruct (step da id').
     - unfold is_extremal. repeat Rdec_full.
-      -- apply sort_max. rewrite <- InA_Leibniz, Spec.support_In. apply Spec.pos_in_config.
-      -- apply sort_max. rewrite <- InA_Leibniz, Spec.support_In. apply Spec.pos_in_config.
+      -- apply sort_max. rewrite <- InA_Leibniz, Spect.support_In. apply Spect.pos_in_config.
+      -- apply sort_max. rewrite <- InA_Leibniz, Spect.support_In. apply Spect.pos_in_config.
       -- apply Rlt_le. change (extreme_center (!! config) < maxi (!! config)). now apply Generic_mid_max_lt.
-    - apply sort_max. rewrite <- InA_Leibniz, Spec.support_In. apply Spec.pos_in_config.
+    - apply sort_max. rewrite <- InA_Leibniz, Spect.support_In. apply Spect.pos_in_config.
 * apply sort_max.
-  rewrite <- Hid, <- InA_Leibniz, Spec.support_In, H. apply Spec.pos_in_config.
+  rewrite <- Hid, <- InA_Leibniz, Spect.support_In, H. apply Spect.pos_in_config.
 Qed.
 
 
 Corollary Generic_extreme_center_same : forall da conf,
-  no_Majority conf -> (Spec.size (!! conf) <> 3)%nat ->
+  no_Majority conf -> (Spect.size (!! conf) <> 3)%nat ->
   extreme_center (!! (round robogram da conf)) = extreme_center (!! conf).
 Proof.
 intros da conf Hmaj Hlen. unfold extreme_center.
@@ -1489,14 +1489,14 @@ now rewrite (Generic_min_same _ Hmaj Hlen), (Generic_max_same _ Hmaj Hlen).
 Qed.
 
 Theorem Generic_min_mult_same : forall da conf,
-  no_Majority conf -> (Spec.size (!! conf) <> 3)%nat ->
+  no_Majority conf -> (Spect.size (!! conf) <> 3)%nat ->
   (!! (round robogram da conf))[mini (!! conf)] = (!! conf)[mini (!! conf)].
 Proof. 
 intros da conf Hmaj Hlen.
 (* We simplify the lhs *)
 rewrite round_simplify_Generic; trivial.
-do 2 rewrite Spec.from_config_spec, Pos.list_spec.
-induction Spec.Names.names as [| id l]; simpl.
+do 2 rewrite Spect.from_config_spec, Pos.list_spec.
+induction Spect.Names.names as [| id l]; simpl.
 * reflexivity.
 * destruct (step da id).
   + repeat Rdec_full.
@@ -1511,14 +1511,14 @@ induction Spec.Names.names as [| id l]; simpl.
 Qed.
 
 Theorem Generic_max_mult_same : forall da conf,
-  no_Majority conf -> (Spec.size (!! conf) <> 3)%nat ->
+  no_Majority conf -> (Spect.size (!! conf) <> 3)%nat ->
   (!! (round robogram da conf))[maxi (!! conf)] = (!! conf)[maxi (!! conf)].
 Proof. 
 intros da conf Hmaj Hlen.
 (* We simplify the lhs *)
 rewrite round_simplify_Generic; trivial.
-do 2 rewrite Spec.from_config_spec, Pos.list_spec.
-induction Spec.Names.names as [| id l]; simpl.
+do 2 rewrite Spect.from_config_spec, Pos.list_spec.
+induction Spect.Names.names as [| id l]; simpl.
 * reflexivity.
 * destruct (step da id).
   + repeat Rdec_full.
@@ -1539,13 +1539,13 @@ Lemma sum3_le_total : forall config pt1 pt2 pt3, pt1 <> pt2 -> pt2 <> pt3 -> pt1
 Proof.
 intros config pt1 pt2 pt3 Hpt12 Hpt23 Hpt13.
 replace N.nG with (N.nG + N.nB) by (unfold N.nB; omega).
-rewrite <- (Spec.cardinal_from_config config).
-rewrite <- (@Spec.add_remove_id pt1 _ (!! config) (reflexivity _)) at 4.
-rewrite Spec.cardinal_add.
-rewrite <- (@Spec.add_remove_id pt2 _ (!! config) (reflexivity _)) at 6.
-rewrite Spec.remove_add_comm, Spec.cardinal_add; trivial.
-rewrite <- (@Spec.add_remove_id pt3 _ (!! config) (reflexivity _)) at 8.
-rewrite Spec.remove_add_comm, Spec.remove_add_comm, Spec.cardinal_add; trivial.
+rewrite <- (Spect.cardinal_from_config config).
+rewrite <- (@Spect.add_remove_id pt1 _ (!! config) (reflexivity _)) at 4.
+rewrite Spect.cardinal_add.
+rewrite <- (@Spect.add_remove_id pt2 _ (!! config) (reflexivity _)) at 6.
+rewrite Spect.remove_add_comm, Spect.cardinal_add; trivial.
+rewrite <- (@Spect.add_remove_id pt3 _ (!! config) (reflexivity _)) at 8.
+rewrite Spect.remove_add_comm, Spect.remove_add_comm, Spect.cardinal_add; trivial.
 omega.
 Qed.
 
@@ -1557,18 +1557,18 @@ intros da config id1 id2 Hid1 Hid2. do 2 rewrite round_simplify.
 destruct (step da id1) eqn:Hmove1; [destruct (step da id2) eqn:Hmove2 |].
 * (* the real case *)
   cbv zeta.
-  destruct (Spec.support (Smax (!! config))) as [| pt [| ? ?]] eqn:Hmaj.
+  destruct (Spect.support (Smax (!! config))) as [| pt [| ? ?]] eqn:Hmaj.
   + (* no robots *)
-    rewrite Spec.support_nil, Smax_empty in Hmaj. elim (spec_non_nil _ Hmaj).
+    rewrite Spect.support_nil, Smax_empty in Hmaj. elim (spec_non_nil _ Hmaj).
   + (* a majority tower *)
     reflexivity.
-  + destruct (Spec.size (!! config) =? 3) eqn:Hlen.
+  + destruct (Spect.size (!! config) =? 3) eqn:Hlen.
     - (* three towers *)
       reflexivity.
     - { (* generic case *)
         rewrite Nat.eqb_neq in Hlen. rename Hmaj into Hmaj'.
         assert (Hmaj : no_Majority  config).
-        { unfold no_Majority. rewrite Spec.size_spec, Hmaj'. simpl. omega. } clear Hmaj'.
+        { unfold no_Majority. rewrite Spect.size_spec, Hmaj'. simpl. omega. } clear Hmaj'.
         destruct (is_extremal (config id1) (!! config)) eqn:Hextreme1.
         + exfalso. unfold moving in Hid1. rewrite filter_In in Hid1. destruct Hid1 as [_ Hid1].
           destruct (R.eq_dec (round robogram da config id1) (config id1)) as [_ | Hneq]; try discriminate.
@@ -1587,19 +1587,19 @@ destruct (step da id1) eqn:Hmove1; [destruct (step da id2) eqn:Hmove2 |].
 Qed.
 
 Lemma towers_elements_3 : forall config pt1 pt2,
-  (Spec.size (!! config) >= 3)%nat ->
-  Spec.In pt1 (!! config) -> Spec.In pt2 (!! config) -> pt1 <> pt2 ->
-  exists pt3, pt1 <> pt3 /\ pt2 <> pt3 /\ Spec.In pt3 (!! config).
+  (Spect.size (!! config) >= 3)%nat ->
+  Spect.In pt1 (!! config) -> Spect.In pt2 (!! config) -> pt1 <> pt2 ->
+  exists pt3, pt1 <> pt3 /\ pt2 <> pt3 /\ Spect.In pt3 (!! config).
 Proof.
 intros config pt1 pt2 Hlen Hpt1 Hpt2 Hdiff12.
-rewrite <- Spec.support_In in *. rewrite Spec.size_spec in Hlen.
+rewrite <- Spect.support_In in *. rewrite Spect.size_spec in Hlen.
 apply (PermutationA_split _) in Hpt1. destruct Hpt1 as [supp1 Hperm].
 rewrite Hperm in Hpt2. inversion_clear Hpt2; try (now elim Hdiff12); []. rename H into Hpt2.
 apply (PermutationA_split _) in Hpt2. destruct Hpt2 as [supp2 Hperm2].
 rewrite Hperm2 in Hperm. rewrite Hperm in Hlen.
 destruct supp2 as [| pt3 supp]; try (now simpl in Hlen; omega); [].
 exists pt3.
-rewrite <- Spec.support_In. assert (Hnodup := Spec.support_NoDupA (!! config)).
+rewrite <- Spect.support_In. assert (Hnodup := Spect.support_NoDupA (!! config)).
 rewrite Hperm in *. inversion_clear Hnodup. inversion_clear H0. repeat split.
 - intro Habs. subst. apply H. now right; left.
 - intro Habs. subst. apply H1. now left.
@@ -1628,8 +1628,8 @@ Proof.
       rewrite <- Rdec_bool_false_iff, <- Rdec_bool_true_iff. apply Hex, Names.In_names. }
     (** We prove a contradiction by showing that the opposite inequality of Hlt holds. *)
     clear Hex. revert Hlt. apply le_not_lt.
-    do 2 rewrite Spec.from_config_spec, Spec.Pos.list_spec.
-    induction Spec.Names.names as [| id l]; simpl; trivial.
+    do 2 rewrite Spect.from_config_spec, Spect.Pos.list_spec.
+    induction Spect.Names.names as [| id l]; simpl; trivial.
     destruct (R.eq_dec (round r da conf id) pt) as [Heq | Heq].
     + destruct (R.eq_dec (conf id) pt); try omega. specialize (Hg id). intuition.
     + destruct (R.eq_dec (conf id) pt); omega.
@@ -1649,9 +1649,9 @@ intros conf da pt. split.
   assert (Hstay : forall id, conf id = pt -> round robogram da conf id = pt).
   { intros id' Hid'. destruct (Rdec (round robogram da conf id') pt) as [Heq | Heq]; trivial.
     assert (Habs := Heq). rewrite <- Hid', <- moving_spec in Habs. apply Hdest in Habs. contradiction. }
-  do 2 rewrite Spec.from_config_spec, Spec.Pos.list_spec.
-  assert (Hin : In id Spec.Names.names) by apply Names.In_names.
-  induction Spec.Names.names as [| id' l]; try (now inversion Hin); [].
+  do 2 rewrite Spect.from_config_spec, Spect.Pos.list_spec.
+  assert (Hin : In id Spect.Names.names) by apply Names.In_names.
+  induction Spect.Names.names as [| id' l]; try (now inversion Hin); [].
   inversion_clear Hin.
   + subst id'. clear IHl. simpl. destruct (R.eq_dec (conf id) pt) as [Heq | Heq].
     - rewrite <- Hid in Heq. now elim Hroundid.
@@ -1674,14 +1674,14 @@ Theorem never_forbidden : forall da conf, ~forbidden conf -> ~forbidden (round r
 Proof.
 intros da conf Hok.
 (* Three cases for the robogram *)
-destruct (Spec.support (Smax (!! conf))) as [| pt [| pt' l']] eqn:Hmaj.
+destruct (Spect.support (Smax (!! conf))) as [| pt [| pt' l']] eqn:Hmaj.
 { (* Absurd case: no robot *)
   intros _. apply (support_Smax_non_nil _ Hmaj). }
 { (* There is a majority tower *)
   rewrite <- MajTower_at_equiv in Hmaj.
   apply Majority_not_forbidden with pt. now apply MajTower_at_forever. }
 { rename Hmaj into Hmaj'.
-  assert (Hmaj : no_Majority conf). { unfold no_Majority. rewrite Spec.size_spec, Hmaj'. simpl. omega. }
+  assert (Hmaj : no_Majority conf). { unfold no_Majority. rewrite Spect.size_spec, Hmaj'. simpl. omega. }
   clear pt pt' l' Hmaj'.
   (* A robot has moved otherwise we have the same configuration before and it is forbidden. *)
   assert (Hnil := no_moving_same_conf robogram da conf).
@@ -1694,19 +1694,19 @@ destruct (Spec.support (Smax (!! conf))) as [| pt [| pt' l']] eqn:Hmaj.
     assert (Hforbidden := Habs). destruct Habs as [HnG [pt1 [pt2 [Hdiff [Hpt1 Hpt2]]]]].
     assert (Hpt : exists pt pt', (pt = pt1 /\ pt' = pt2 \/ pt = pt2  /\ pt' = pt1)
                                   /\ round robogram da conf rmove = pt).
-    { assert (Hperm : Permutation (Spec.support (!! (round robogram da conf))) (pt1 :: pt2 :: nil)).
+    { assert (Hperm : Permutation (Spect.support (!! (round robogram da conf))) (pt1 :: pt2 :: nil)).
       { symmetry. apply NoDup_Permutation_bis.
         + repeat constructor.
           - intro Habs. inversion Habs. now elim Hdiff. now inversion H.
           - intro Habs. now inversion Habs.
-        + rewrite <- NoDupA_Leibniz. apply Spec.support_NoDupA.
-        + simpl. now rewrite <- Spec.size_spec, forbidden_support_length.
+        + rewrite <- NoDupA_Leibniz. apply Spect.support_NoDupA.
+        + simpl. now rewrite <- Spect.size_spec, forbidden_support_length.
         + intros pt Hpt. inversion_clear Hpt.
-          - subst. rewrite <- InA_Leibniz, Spec.support_spec. unfold Spec.In. rewrite Hpt1. apply half_size_pos.
-          - inversion H; (now inversion H0) || subst. rewrite <- InA_Leibniz, Spec.support_spec.
-            unfold Spec.In. rewrite Hpt2. apply half_size_pos. }
+          - subst. rewrite <- InA_Leibniz, Spect.support_spec. unfold Spect.In. rewrite Hpt1. apply half_size_pos.
+          - inversion H; (now inversion H0) || subst. rewrite <- InA_Leibniz, Spect.support_spec.
+            unfold Spect.In. rewrite Hpt2. apply half_size_pos. }
       assert (Hpt : In (round robogram da conf rmove) (pt1 :: pt2 :: nil)).
-      { rewrite <- Hperm. rewrite <- InA_Leibniz, Spec.support_In. apply Spec.pos_in_config. }
+      { rewrite <- Hperm. rewrite <- InA_Leibniz, Spect.support_In. apply Spect.pos_in_config. }
       inversion_clear Hpt; try (now exists pt1, pt2; eauto); [].
       inversion_clear H; now exists pt2, pt1; eauto. }
     destruct Hpt as [pt [pt' [Hpt Hrmove_pt]]].
@@ -1727,15 +1727,15 @@ destruct (Spec.support (Smax (!! conf))) as [| pt [| pt' l']] eqn:Hmaj.
         symmetry.
         apply Hdest. rewrite moving_spec. assumption. }
     assert (Hlt : forall p, p <> pt' -> (!! conf)[p] < div2 N.nG).
-    { assert (Hpt'_in : Spec.In pt' (!! conf)).
-      { unfold Spec.In. eapply lt_le_trans; try eassumption. apply half_size_pos. }
+    { assert (Hpt'_in : Spect.In pt' (!! conf)).
+      { unfold Spect.In. eapply lt_le_trans; try eassumption. apply half_size_pos. }
       assert (Hle := not_forbidden_not_majority_length Hmaj Hok).
       intros p Hp. apply Nat.nle_gt. intro Habs. apply (lt_irrefl N.nG).
       destruct (@towers_elements_3 conf pt' p Hle Hpt'_in) as [pt3' [Hdiff13 [Hdiff23 Hpt3_in]]]; trivial.
       + apply lt_le_trans with (div2 N.nG); try assumption. apply half_size_pos.
       + auto.
       + eapply lt_le_trans; try apply (sum3_le_total conf Hp Hdiff13 Hdiff23); [].
-        unfold Spec.In in Hpt3_in. rewrite (even_double N.nG), Nat.double_twice. omega.
+        unfold Spect.In in Hpt3_in. rewrite (even_double N.nG), Nat.double_twice. omega.
         now rewrite Even.even_equiv. }
     assert (Hmaj' : MajTower_at pt' conf).
     { intros x Hx. apply lt_le_trans with (div2 N.nG); trivial. now apply Hlt. }
@@ -1810,15 +1810,15 @@ End WfLexicographic_Product.
 
 Definition conf_to_NxN conf :=
   let s := !! conf in
-  match Spec.support (Smax s) with
+  match Spect.support (Smax s) with
     | nil => (0,0)
     | pt :: nil => (1, N.nG - s[pt])
     | _ :: _ :: _ =>
-        if beq_nat (Spec.size s) 3
-        then (2, N.nG - s[nth 1 (sort (Spec.support s)) 0%R])
+        if beq_nat (Spect.size s) 3
+        then (2, N.nG - s[nth 1 (sort (Spect.support s)) 0%R])
         else (3, N.nG - (s[extreme_center s]
-                         + s[hd 0%R (sort  (Spec.support s))]
-                         + s[last (sort  (Spec.support s)) 0%R]))
+                         + s[hd 0%R (sort  (Spect.support s))]
+                         + s[last (sort  (Spect.support s)) 0%R]))
   end.
 
 Require Import Inverse_Image.
@@ -1836,15 +1836,15 @@ Qed.
 Instance conf_to_NxN_compat: Proper (Pos.eq ==> eq * eq) conf_to_NxN.
 Proof.
 intros pos1 pos2 Heq. unfold conf_to_NxN.
-assert (Hperm : PermutationA R.eq (Spec.support (Smax (!! pos1)))
-                                  (Spec.support (Smax (!! pos2)))) by now rewrite Heq.
-destruct (Spec.support (Smax (!! pos2))) as [| pt [| ? ?]] eqn:Hsupp.
+assert (Hperm : PermutationA R.eq (Spect.support (Smax (!! pos1)))
+                                  (Spect.support (Smax (!! pos2)))) by now rewrite Heq.
+destruct (Spect.support (Smax (!! pos2))) as [| pt [| ? ?]] eqn:Hsupp.
 + symmetry in Hperm. apply (PermutationA_nil _) in Hperm. rewrite Hperm. reflexivity.
 + apply (PermutationA_length1 _) in Hperm. destruct Hperm as [y [Hy Hperm]].
   rewrite Hperm, <- Hy, Heq. reflexivity.
 + apply (PermutationA_length _) in Hperm.
-  destruct (Spec.support (Smax (!! pos1))) as [| ? [| ? ?]]; try discriminate Hperm.
-  rewrite Heq. destruct (Spec.size (!! pos2) =? 3); rewrite Heq; reflexivity.
+  destruct (Spect.support (Smax (!! pos1))) as [| ? [| ? ?]]; try discriminate Hperm.
+  rewrite Heq. destruct (Spect.size (!! pos2) =? 3); rewrite Heq; reflexivity.
 Qed.
 
 Instance lexprod_compat: Proper (eq * eq ==> eq * eq ==> iff) (lexprod lt lt).
@@ -1865,7 +1865,7 @@ Proof.
 Qed.
 
 Lemma conf_to_NxN_nil_spec : forall conf,
-  Spec.support (Smax (!! conf)) = nil -> conf_to_NxN conf = (0, 0).
+  Spect.support (Smax (!! conf)) = nil -> conf_to_NxN conf = (0, 0).
 Proof. intros conf Heq. unfold conf_to_NxN. rewrite Heq. reflexivity. Qed.
 
 Lemma conf_to_NxN_Majority_spec : forall conf pt,
@@ -1880,61 +1880,61 @@ Qed.
 
 Lemma conf_to_NxN_Three_spec : forall conf,
   no_Majority conf ->
-  Spec.size (!! conf) = 3 ->
-  conf_to_NxN conf = (2, N.nG - (!! conf)[nth 1 (sort (Spec.support (!! conf))) 0%R]).
+  Spect.size (!! conf) = 3 ->
+  conf_to_NxN conf = (2, N.nG - (!! conf)[nth 1 (sort (Spect.support (!! conf))) 0%R]).
 Proof.
 intros conf Hmaj Hlen. unfold conf_to_NxN.
-unfold no_Majority in Hmaj. rewrite Spec.size_spec in Hmaj.
-destruct (Spec.support (Smax (!! conf))) as [| ? [| ? ?]]; simpl in Hmaj; try omega.
+unfold no_Majority in Hmaj. rewrite Spect.size_spec in Hmaj.
+destruct (Spect.support (Smax (!! conf))) as [| ? [| ? ?]]; simpl in Hmaj; try omega.
 rewrite <- Nat.eqb_eq in Hlen. rewrite Hlen. reflexivity.
 Qed.
 
 Lemma conf_to_NxN_Generic_spec : forall conf,
   no_Majority conf ->
-  Spec.size (!!  conf) <> 3 ->
+  Spect.size (!!  conf) <> 3 ->
     conf_to_NxN conf = 
     (3, N.nG - ((!! conf)[extreme_center (!! conf)]
                 + (!! conf)[mini (!! conf)]
                 + (!! conf)[maxi (!! conf)])).
 Proof.
 intros conf Hmaj Hlen. unfold conf_to_NxN.
-unfold no_Majority in Hmaj. rewrite Spec.size_spec in Hmaj.
-destruct (Spec.support (Smax (!! conf))) as [| ? [| ? ?]]; simpl in Hmaj; try omega.
+unfold no_Majority in Hmaj. rewrite Spect.size_spec in Hmaj.
+destruct (Spect.support (Smax (!! conf))) as [| ? [| ? ?]]; simpl in Hmaj; try omega.
 rewrite <- Nat.eqb_neq in Hlen. rewrite Hlen. reflexivity.
 Qed.
 
 Lemma multiplicity_le_nG : forall pt conf, (!! conf)[pt] <= N.nG.
 Proof.
 intros pt conf. etransitivity.
-- apply Spec.cardinal_lower.
-- rewrite Spec.cardinal_from_config. unfold N.nB. omega.
+- apply Spect.cardinal_lower.
+- rewrite Spect.cardinal_from_config. unfold N.nB. omega.
 Qed.
 
 (* When we only have three towers, the new configuration does not create new positions. *)
 Lemma support_round_Three_incl : forall conf da,
   no_Majority conf ->
-  Spec.size (!!  conf) = 3 ->
-  incl (Spec.support (!! (round robogram da conf)))
-       (Spec.support (!! conf)).
+  Spect.size (!!  conf) = 3 ->
+  incl (Spect.support (!! (round robogram da conf)))
+       (Spect.support (!! conf)).
 Proof.
 intros config da Hmaj Hlen pt Hin.
-rewrite <- InA_Leibniz, Spec.support_In, Spec.from_config_In in Hin.
+rewrite <- InA_Leibniz, Spect.support_In, Spect.from_config_In in Hin.
 destruct Hin as [id Hid]. rewrite round_simplify_Three in Hid; trivial.
 destruct (step da id).
 + rewrite <- Hid. setoid_rewrite Permuted_sort at 3. apply nth_In.
-  rewrite <- Permuted_sort, <- Spec.size_spec, Hlen. omega.
-+ rewrite <- InA_Leibniz, Spec.support_In, <- Hid. apply Spec.pos_in_config.
+  rewrite <- Permuted_sort, <- Spect.size_spec, Hlen. omega.
++ rewrite <- InA_Leibniz, Spect.support_In, <- Hid. apply Spect.pos_in_config.
 Qed.
 
 Corollary support_decrease : forall conf da,
   no_Majority conf ->
-  Spec.size (!! conf) = 3 ->
-  Spec.size (!! (round robogram da conf)) <= 3.
+  Spect.size (!! conf) = 3 ->
+  Spect.size (!! (round robogram da conf)) <= 3.
 Proof.
 intros conf da Hmaj Hlen. rewrite <- Hlen.
 generalize (support_round_Three_incl da Hmaj Hlen).
-rewrite <- inclA_Leibniz, Spec.size_spec, Spec.size_spec.
-apply (NoDupA_inclA_length _). apply Spec.support_NoDupA.
+rewrite <- inclA_Leibniz, Spect.size_spec, Spect.size_spec.
+apply (NoDupA_inclA_length _). apply Spect.support_NoDupA.
 Qed.
 
 Theorem round_lt_conf : forall da conf,
@@ -1946,7 +1946,7 @@ apply not_nil_In in Hmove. destruct Hmove as [gmove Hmove].
 assert (Hstep : step da gmove <> None).
 { apply moving_active in Hmove. now rewrite active_spec in Hmove. }
 rewrite moving_spec in Hmove.
-destruct (Spec.support (Smax (!! conf))) as [| pt [| ? ?]] eqn:Hmaj.
+destruct (Spect.support (Smax (!! conf))) as [| pt [| ? ?]] eqn:Hmaj.
 * (* No robots *)
   elim (support_Smax_non_nil _ Hmaj).
 * (* A majority tower *)
@@ -1962,38 +1962,38 @@ destruct (Spec.support (Smax (!! conf))) as [| pt [| ? ?]] eqn:Hmaj.
   rewrite increase_move_iff. eauto.
 * rename Hmaj into Hmaj'.
   assert (Hmaj : no_Majority conf).
-  { unfold no_Majority. rewrite Spec.size_spec, Hmaj'. simpl. omega. } clear Hmaj'.
-  destruct (eq_nat_dec (Spec.size (!! conf)) 3) as [Hlen | Hlen].
+  { unfold no_Majority. rewrite Spect.size_spec, Hmaj'. simpl. omega. } clear Hmaj'.
+  destruct (eq_nat_dec (Spect.size (!! conf)) 3) as [Hlen | Hlen].
   + (* Three towers case *)
     red. rewrite (conf_to_NxN_Three_spec Hmaj Hlen).
-    destruct (Spec.support (Smax (!! (round robogram da conf)))) as [| pt' [| ? ?]] eqn:Hmaj'.
+    destruct (Spect.support (Smax (!! (round robogram da conf)))) as [| pt' [| ? ?]] eqn:Hmaj'.
     - rewrite (conf_to_NxN_nil_spec _ Hmaj'). apply left_lex. omega.
     - rewrite <- MajTower_at_equiv in Hmaj'. rewrite (conf_to_NxN_Majority_spec Hmaj'). apply left_lex. omega.
     - rename Hmaj' into Hmaj''.
       assert (Hmaj' : no_Majority (round robogram da conf)).
-      { unfold no_Majority. rewrite Spec.size_spec, Hmaj''. simpl. omega. } clear Hmaj''.
-      assert (Hlen' : Spec.size (!! (round robogram da conf)) = 3).
+      { unfold no_Majority. rewrite Spect.size_spec, Hmaj''. simpl. omega. } clear Hmaj''.
+      assert (Hlen' : Spect.size (!! (round robogram da conf)) = 3).
       { apply le_antisym.
         + apply (support_decrease _ Hmaj Hlen).
         + apply (not_forbidden_not_majority_length Hmaj'). now apply never_forbidden. }
       rewrite (conf_to_NxN_Three_spec Hmaj' Hlen'). apply right_lex.
       rewrite <- Hlen in Hlen'.
-      assert (Hperm : Permutation (Spec.support (!! (round robogram da conf)))
-                                  (Spec.support (!! conf))).
+      assert (Hperm : Permutation (Spect.support (!! (round robogram da conf)))
+                                  (Spect.support (!! conf))).
       { rewrite <- PermutationA_Leibniz. apply (NoDupA_inclA_length_PermutationA _).
-        - apply Spec.support_NoDupA.
-        - apply Spec.support_NoDupA.
+        - apply Spect.support_NoDupA.
+        - apply Spect.support_NoDupA.
         - rewrite inclA_Leibniz. eapply support_round_Three_incl; eassumption.
-        - do 2 rewrite <- Spec.size_spec. assumption. }
+        - do 2 rewrite <- Spect.size_spec. assumption. }
       rewrite Hperm.
-      assert (Hup := multiplicity_le_nG (nth 1 (sort (Spec.support (!! conf))) 0%R)
+      assert (Hup := multiplicity_le_nG (nth 1 (sort (Spect.support (!! conf))) 0%R)
                                         (round robogram da conf)).
-      cut (Spec.multiplicity
-              (nth 1 (sort (Spec.support (!! conf))) 0%R)
+      cut (Spect.multiplicity
+              (nth 1 (sort (Spect.support (!! conf))) 0%R)
               (!! (round robogram da conf))
             >
-            Spec.multiplicity
-              (nth 1 (sort (Spec.support (!! conf))) 0%R)
+            Spect.multiplicity
+              (nth 1 (sort (Spect.support (!! conf))) 0%R)
               (!! conf)). omega.
       unfold gt. rewrite increase_move_iff.
       exists gmove. split; trivial.
@@ -2002,13 +2002,13 @@ destruct (Spec.support (Smax (!! conf))) as [| pt [| ? ?]] eqn:Hmaj.
       destruct gmove eqn:Hid; trivial.
   + (* Generic case *)
     red. rewrite (conf_to_NxN_Generic_spec Hmaj Hlen).
-    destruct (Spec.support (Smax (!! (round robogram da conf)))) as [| pt' [| ? ?]] eqn:Hmaj'.
+    destruct (Spect.support (Smax (!! (round robogram da conf)))) as [| pt' [| ? ?]] eqn:Hmaj'.
     - rewrite (conf_to_NxN_nil_spec _ Hmaj'). apply left_lex. omega.
     - rewrite <- MajTower_at_equiv in Hmaj'. rewrite (conf_to_NxN_Majority_spec Hmaj'). apply left_lex. omega.
     - { rename Hmaj' into Hmaj''.
         assert (Hmaj' : no_Majority (round robogram da conf)).
-        { unfold no_Majority. rewrite Spec.size_spec, Hmaj''. simpl. omega. } clear Hmaj''.
-        destruct (eq_nat_dec (Spec.size (!! (round robogram da conf))) 3)
+        { unfold no_Majority. rewrite Spect.size_spec, Hmaj''. simpl. omega. } clear Hmaj''.
+        destruct (eq_nat_dec (Spect.size (!! (round robogram da conf))) 3)
         as [Hlen' | Hlen'].
         + rewrite (conf_to_NxN_Three_spec Hmaj' Hlen'). apply left_lex. omega.
         + rewrite (conf_to_NxN_Generic_spec Hmaj' Hlen'). apply right_lex.
@@ -2122,13 +2122,13 @@ Qed.
 
 Lemma not_forbidden_gathered_Majority_size : forall config id,
   ~forbidden config -> ~gathered_at (config id) config -> no_Majority config ->
-  Spec.size (!! config) >= 3.
+  Spect.size (!! config) >= 3.
 Proof.
 intros config id Hforbidden Hgather Hmaj.
-assert (Spec.size (!! config) > 1).
+assert (Spect.size (!! config) > 1).
 { unfold no_Majority in Hmaj. eapply lt_le_trans; try eassumption; []. now rewrite Smax_subset. }
 rewrite forbidden_equiv in Hforbidden.
-destruct (Spec.size (!! config)) as [| [| [| n]]]; omega || tauto.
+destruct (Spect.size (!! config)) as [| [| [| n]]]; omega || tauto.
 Qed.
 
 (** Given a non-gathered, non forbidden position, then some robot will move some day *)
@@ -2136,7 +2136,7 @@ Theorem OneMustMove : forall config id, ~ forbidden config -> ~gathered_at (conf
   exists gmove, forall da, In gmove (active da) -> In gmove (moving robogram da config).
 Proof.
 intros config id Hforbidden Hgather.
-destruct (Spec.support (Smax (!! config))) as [| pt [| ? ?]] eqn:Hmaj.
+destruct (Spect.support (Smax (!! config))) as [| pt [| ? ?]] eqn:Hmaj.
 * elim (support_Smax_non_nil _ Hmaj).
 * rewrite <- MajTower_at_equiv in Hmaj.
   apply not_gathered_generalize with _ _ pt in Hgather.
@@ -2144,34 +2144,34 @@ destruct (Spec.support (Smax (!! config))) as [| pt [| ? ?]] eqn:Hmaj.
   exists gmove. intros da Hactive. rewrite active_spec in Hactive. rewrite moving_spec.
   rewrite (round_simplify_Majority _ Hmaj). destruct (step da gmove); auto; now elim Hactive.
 * rename Hmaj into Hmaj'.
-  assert (Hmaj : no_Majority config). { unfold no_Majority. rewrite Spec.size_spec, Hmaj'. simpl. omega. }
+  assert (Hmaj : no_Majority config). { unfold no_Majority. rewrite Spect.size_spec, Hmaj'. simpl. omega. }
   clear Hmaj' pt e l.
-  destruct (eq_nat_dec (Spec.size (!! config)) 3) as [Hlen| Hlen].
+  destruct (eq_nat_dec (Spect.size (!! config)) 3) as [Hlen| Hlen].
   + apply not_gathered_generalize with _ _ (middle (!! config)) in Hgather.
     apply not_gathered_exists in Hgather. destruct Hgather as [gmove Hmove].
     exists gmove. intros da Hactive. rewrite active_spec in Hactive. rewrite moving_spec.
     rewrite (round_simplify_Three _ Hmaj Hlen). destruct (step da gmove); auto; now elim Hactive.
-  + assert (Hle : Spec.size (!! config) >= 4).
+  + assert (Hle : Spect.size (!! config) >= 4).
     { hnf. apply le_neq_lt.
       - now apply not_forbidden_gathered_Majority_size with id.
       - auto. }
-    rewrite Spec.size_spec, Permuted_sort in Hle.
-    destruct (sort (Spec.support (!! config))) as [| pt1 [| pt2 [| pt3 [| pt4 l]]]] eqn:Hsup;
+    rewrite Spect.size_spec, Permuted_sort in Hle.
+    destruct (sort (Spect.support (!! config))) as [| pt1 [| pt2 [| pt3 [| pt4 l]]]] eqn:Hsup;
     simpl in Hle; omega || clear Hle.
-    assert (Hex : exists pt, Spec.In pt (!! config) /\ pt <> extreme_center (!! config)
+    assert (Hex : exists pt, Spect.In pt (!! config) /\ pt <> extreme_center (!! config)
                              /\ pt <> mini (!! config) /\ pt <> maxi (!! config)).
     { assert (Hmini : mini (!! config) = pt1). { unfold mini. now rewrite Hsup. }
       assert (Hmaxi : In (maxi (!! config)) (pt4 :: l)).
       { unfold maxi. rewrite Hsup. change (In (last (pt4 :: l) 0%R) (pt4 :: l)). apply last_In. discriminate. }
-      assert (Hnodup := Spec.support_NoDupA (!! config)).
+      assert (Hnodup := Spect.support_NoDupA (!! config)).
       rewrite NoDupA_Leibniz, Permuted_sort, Hsup in Hnodup.
       inversion_clear Hnodup. inversion_clear H0. inversion_clear H2.
       destruct (Rdec pt2 (extreme_center (!! config))) as [Heq | Heq]; subst.
       - exists pt3. repeat split; try now intro; subst; intuition.
-        rewrite <- Spec.support_In, InA_Leibniz, Permuted_sort, Hsup. intuition.
+        rewrite <- Spect.support_In, InA_Leibniz, Permuted_sort, Hsup. intuition.
       - exists pt2. repeat split; try now intro; subst; intuition.
-        rewrite <- Spec.support_In, InA_Leibniz, Permuted_sort, Hsup. intuition. }
-    destruct Hex as [pt [Hin Hmove]]. rewrite Spec.from_config_In in Hin.
+        rewrite <- Spect.support_In, InA_Leibniz, Permuted_sort, Hsup. intuition. }
+    destruct Hex as [pt [Hin Hmove]]. rewrite Spect.from_config_In in Hin.
     destruct Hin as [gmove Heq]. rewrite <- Heq in Hmove.
     exists gmove. intros da Hactive. rewrite active_spec in Hactive. rewrite moving_spec.
     rewrite (round_simplify_Generic _ Hmaj Hlen). destruct (step da gmove); auto.
@@ -2204,13 +2204,13 @@ intros da conf pt Hgather. rewrite (round_simplify_Majority).
 + intro g. destruct (step da (Good g)); reflexivity || apply Hgather.
 + intros pt' Hdiff.
   assert (H0 : (!! conf)[pt'] = 0).
-  { rewrite Spec.from_config_spec, Spec.Pos.list_spec.
-    induction Spec.Names.names as [| id l].
+  { rewrite Spect.from_config_spec, Spect.Pos.list_spec.
+    induction Spect.Names.names as [| id l].
     + reflexivity.
     + unfold R.eq_dec, Rdef.eq_dec in *. simpl. Rdec_full.
       - elim Hdiff. rewrite <- Heq. destruct id as [g | b]. apply Hgather. apply Fin.case0. exact b.
       - apply IHl. }
-  rewrite H0. specialize (Hgather g1). rewrite <- Hgather. apply Spec.pos_in_config.
+  rewrite H0. specialize (Hgather g1). rewrite <- Hgather. apply Spect.pos_in_config.
 Qed.
 
 Lemma gathered_at_dec : forall conf pt, {gathered_at pt conf} + {~gathered_at pt conf}.
@@ -2260,4 +2260,3 @@ Qed.
 Print Assumptions Gathering_in_R.
 
 End GatheringinR.
-
